src/coq/Semantics/InfiniteToFinite/LangRefine.v
@@ -7373,6 +7373,11 @@ Qed.
         reflexivity.
   Qed.
 
+  Definition uvalue_concretize_u_fin_inf_inclusion uv_inf uv_fin :=
+    forall res,
+      IS2.MEM.CP.CONC.concretize_u uv_fin res ->
+      IS1.MEM.CP.CONC.concretize_u uv_inf (fmap fin_to_inf_dvalue res).
+
   Definition uvalue_concretize_fin_inf_inclusion uv_inf uv_fin :=
     forall dv_fin,
       IS2.MEM.CP.CONC.concretize uv_fin dv_fin ->
@@ -8252,6 +8257,345 @@ Qed.
     }
   Admitted.
 
+  Lemma fin_to_inf_dvalue_array :
+    forall elts,
+      fin_to_inf_dvalue (DVALUE_Array elts) =
+        DVCrev.DV2.DVALUE_Array (map fin_to_inf_dvalue elts).
+  Proof.
+    induction elts.
+    - cbn.
+      unfold fin_to_inf_dvalue.
+      break_match_goal; clear Heqs; destruct p; clear e0;
+        cbn in e; subst; inv e.
+      auto.
+    - unfold fin_to_inf_dvalue in *.
+      break_match_goal; clear Heqs; destruct p; clear e0;
+        cbn in e; subst; inv e.
+      break_match_hyp_inv.
+      break_match_hyp_inv.
+      break_match_hyp_inv.
+      rewrite map_cons.
+
+      break_match_hyp_inv; clear Heqs; destruct p; clear e0.
+      cbn in e; subst; inv e.
+
+      break_match_hyp_inv.
+      inv Heqo.
+
+      break_match_goal; clear Heqs; destruct p; clear e0.
+      rewrite Heqo0 in e.
+      inv e.
+      auto.
+  Qed.
+
+  Lemma fin_to_inf_dvalue_vector :
+    forall elts,
+      fin_to_inf_dvalue (DVALUE_Vector elts) =
+        DVCrev.DV2.DVALUE_Vector (map fin_to_inf_dvalue elts).
+  Proof.
+    induction elts.
+    - cbn.
+      unfold fin_to_inf_dvalue.
+      break_match_goal; clear Heqs; destruct p; clear e0;
+        cbn in e; subst; inv e.
+      auto.
+    - unfold fin_to_inf_dvalue in *.
+      break_match_goal; clear Heqs; destruct p; clear e0;
+        cbn in e; subst; inv e.
+      break_match_hyp_inv.
+      break_match_hyp_inv.
+      break_match_hyp_inv.
+      rewrite map_cons.
+
+      break_match_hyp_inv; clear Heqs; destruct p; clear e0.
+      cbn in e; subst; inv e.
+
+      break_match_hyp_inv.
+
+      break_match_goal; clear Heqs; destruct p; clear e0.
+      rewrite Heqo0 in e.
+      inv e.
+
+      inv Heqo.
+      auto.
+  Qed.
+
+  Lemma fin_to_inf_dvalue_i1 :
+    forall x,
+      fin_to_inf_dvalue (DVALUE_I1 x) =
+        DVCrev.DV2.DVALUE_I1 x.
+  Proof.
+    intros x.
+    unfold fin_to_inf_dvalue.
+    break_match_goal; clear Heqs; destruct p; clear e0;
+      cbn in e; subst; inv e.
+    auto.
+  Qed.
+
+  Lemma fin_to_inf_dvalue_i8 :
+    forall x,
+      fin_to_inf_dvalue (DVALUE_I8 x) =
+        DVCrev.DV2.DVALUE_I8 x.
+  Proof.
+    intros x.
+    unfold fin_to_inf_dvalue.
+    break_match_goal; clear Heqs; destruct p; clear e0;
+      cbn in e; subst; inv e.
+    auto.
+  Qed.
+
+  Lemma fin_to_inf_dvalue_i32 :
+    forall x,
+      fin_to_inf_dvalue (DVALUE_I32 x) =
+        DVCrev.DV2.DVALUE_I32 x.
+  Proof.
+    intros x.
+    unfold fin_to_inf_dvalue.
+    break_match_goal; clear Heqs; destruct p; clear e0;
+      cbn in e; subst; inv e.
+    auto.
+  Qed.
+
+  Lemma fin_to_inf_dvalue_i64 :
+    forall x,
+      fin_to_inf_dvalue (DVALUE_I64 x) =
+        DVCrev.DV2.DVALUE_I64 x.
+  Proof.
+    intros x.
+    unfold fin_to_inf_dvalue.
+    break_match_goal; clear Heqs; destruct p; clear e0;
+      cbn in e; subst; inv e.
+    auto.
+  Qed.
+
+  Definition intptr_fin_inf (x : IP.intptr) : IS1.LP.IP.intptr.
+    pose proof intptr_convert_succeeds x.
+    destruct H.
+    apply x0.
+  Defined.
+
+  Lemma fin_to_inf_dvalue_iptr :
+    forall x,
+      fin_to_inf_dvalue (DVALUE_IPTR x) =
+        DVCrev.DV2.DVALUE_IPTR (intptr_fin_inf x).
+  Proof.
+    intros x.
+    unfold fin_to_inf_dvalue.
+    break_match_goal; clear Heqs; destruct p; clear e0;
+      cbn in e; subst; inv e.
+
+    pose proof intptr_convert_succeeds x.
+    destruct H.
+    rewrite e in H0.
+    inv H0.
+
+    unfold intptr_fin_inf.
+    break_match_goal.
+    clear Heqs.
+    congruence.
+  Qed.
+
+  (* TODO: Should we move this? *)
+  Definition addr_refine addr_inf (addr_fin : addr) := AC1.addr_convert addr_inf = NoOom addr_fin.
+
+  (* TODO: Should we move this? *)
+  Definition fin_to_inf_addr (a : addr) : IS1.LP.ADDR.addr.
+    unfold FinAddr.addr in a.
+    unfold FiniteAddresses.Iptr in a.
+    pose proof ACS.addr_convert_succeeds a as [a' _].
+    exact a'.
+  Defined.
+
+  (* TODO: Move this *)
+  Lemma addr_refine_fin_to_inf_addr :
+    forall addr_fin,
+      addr_refine (fin_to_inf_addr addr_fin) addr_fin.
+  Proof.
+    intros addr_fin.
+    red. unfold fin_to_inf_addr.
+    break_match_goal.
+    clear Heqs.
+    apply ACS.addr_convert_safe in e.
+    auto.
+  Qed.
+
+  Lemma addr_convert_fin_to_inf_addr :
+    forall addr_fin,
+      AC1.addr_convert (fin_to_inf_addr addr_fin) = NoOom addr_fin.
+  Proof.
+    intros addr_fin.
+    unfold fin_to_inf_addr in *.
+    destruct (ACS.addr_convert_succeeds addr_fin).
+    apply ACS.addr_convert_safe in e.
+    auto.
+  Qed.
+
+  Lemma fin_to_inf_dvalue_addr :
+    forall a,
+      fin_to_inf_dvalue (DVALUE_Addr a) =
+        DVCrev.DV2.DVALUE_Addr (fin_to_inf_addr a).
+  Proof.
+    intros a.
+    unfold fin_to_inf_dvalue.
+    break_match_goal; clear Heqs; destruct p; clear e0.
+    cbn in e.
+    break_match_hyp_inv.
+    unfold fin_to_inf_addr.
+    break_match_goal.
+    clear Heqs.
+    rewrite Heqo in e.
+    inv e.
+    auto.
+  Qed.
+
+  Lemma fin_to_inf_dvalue_float :
+    forall f,
+      fin_to_inf_dvalue (DVALUE_Float f) =
+        DVCrev.DV2.DVALUE_Float f.
+  Proof.
+    intros a.
+    unfold fin_to_inf_dvalue.
+    break_match_goal; clear Heqs; destruct p; clear e0.
+    cbn in e. inv e.
+    reflexivity.
+  Qed.
+
+  Lemma fin_to_inf_dvalue_double :
+    forall f,
+      fin_to_inf_dvalue (DVALUE_Double f) =
+        DVCrev.DV2.DVALUE_Double f.
+  Proof.
+    intros a.
+    unfold fin_to_inf_dvalue.
+    break_match_goal; clear Heqs; destruct p; clear e0.
+    cbn in e. inv e.
+    reflexivity.
+  Qed.
+
+  Lemma fin_to_inf_dvalue_poison :
+    forall t,
+      fin_to_inf_dvalue (DVALUE_Poison t) =
+        DVCrev.DV2.DVALUE_Poison t.
+  Proof.
+    intros x.
+    unfold fin_to_inf_dvalue.
+    break_match_goal; clear Heqs; destruct p; clear e0;
+      cbn in e; subst; inv e.
+    auto.
+  Qed.
+
+  Lemma fin_to_inf_dvalue_oom :
+    forall t,
+      fin_to_inf_dvalue (DVALUE_Oom t) =
+        DVCrev.DV2.DVALUE_Oom t.
+  Proof.
+    intros x.
+    unfold fin_to_inf_dvalue.
+    break_match_goal; clear Heqs; destruct p; clear e0;
+      cbn in e; subst; inv e.
+    auto.
+  Qed.
+
+  Lemma fin_to_inf_dvalue_none :
+      fin_to_inf_dvalue DVALUE_None =
+        DVCrev.DV2.DVALUE_None.
+  Proof.
+    unfold fin_to_inf_dvalue.
+    break_match_goal; clear Heqs; destruct p; clear e0;
+      cbn in e; subst; inv e.
+    auto.
+  Qed.
+
+  (* TODO: Move this *)
+  Lemma sizeof_dtyp_fin_inf :
+    forall t,
+      IS1.LP.SIZEOF.sizeof_dtyp t = SIZEOF.sizeof_dtyp t.
+  Proof.
+    (* Need to expose more stuff to be able to prove this *)
+  Admitted.
+
+  Lemma fin_to_inf_dvalue_struct :
+    forall elts,
+      fin_to_inf_dvalue (DVALUE_Struct elts) =
+        DVCrev.DV2.DVALUE_Struct (map fin_to_inf_dvalue elts).
+  Proof.
+    induction elts.
+    - cbn.
+      unfold fin_to_inf_dvalue.
+      break_match_goal; clear Heqs; destruct p; clear e0;
+        cbn in e; subst; inv e.
+      auto.
+    - unfold fin_to_inf_dvalue in *.
+      break_match_goal; clear Heqs; destruct p; clear e0;
+        cbn in e; subst; inv e.
+      break_match_hyp_inv.
+      break_match_hyp_inv.
+      break_match_hyp_inv.
+
+      break_match_hyp_inv; clear Heqs; destruct p; clear e0.
+      cbn in e; subst; inv e.
+
+      break_match_hyp_inv.
+      rewrite map_cons.
+      inv Heqo.
+
+      break_match_goal; clear Heqs; destruct p; clear e0.
+      rewrite Heqo0 in e.
+      inv e.
+      auto.
+  Qed.
+
+  Lemma fin_to_inf_dvalue_packed_struct :
+    forall elts,
+      fin_to_inf_dvalue (DVALUE_Packed_struct elts) =
+        DVCrev.DV2.DVALUE_Packed_struct (map fin_to_inf_dvalue elts).
+  Proof.
+    induction elts.
+    - cbn.
+      unfold fin_to_inf_dvalue.
+      break_match_goal; clear Heqs; destruct p; clear e0;
+        cbn in e; subst; inv e.
+      auto.
+    - unfold fin_to_inf_dvalue in *.
+      break_match_goal; clear Heqs; destruct p; clear e0;
+        cbn in e; subst; inv e.
+      break_match_hyp_inv.
+      break_match_hyp_inv.
+      break_match_hyp_inv.
+
+      break_match_hyp_inv; clear Heqs; destruct p; clear e0.
+      cbn in e; subst; inv e.
+
+      break_match_hyp_inv.
+      rewrite map_cons.
+      inv Heqo.
+
+      break_match_goal; clear Heqs; destruct p; clear e0.
+      rewrite Heqo0 in e.
+      inv e.
+      auto.
+  Qed.
+
+  Ltac rewrite_fin_to_inf_dvalue :=
+    repeat
+      first
+      [ rewrite fin_to_inf_dvalue_i1
+      | rewrite fin_to_inf_dvalue_i8
+      | rewrite fin_to_inf_dvalue_i32
+      | rewrite fin_to_inf_dvalue_i64
+      | rewrite fin_to_inf_dvalue_iptr
+      | rewrite fin_to_inf_dvalue_addr
+      | rewrite fin_to_inf_dvalue_float
+      | rewrite fin_to_inf_dvalue_double
+      | rewrite fin_to_inf_dvalue_poison
+      | rewrite fin_to_inf_dvalue_oom
+      | rewrite fin_to_inf_dvalue_none
+      | rewrite fin_to_inf_dvalue_array
+      | rewrite fin_to_inf_dvalue_vector
+      | rewrite fin_to_inf_dvalue_struct
+      | rewrite fin_to_inf_dvalue_packed_struct
+      ].
+
   Lemma eval_int_icmp_fin_inf :
     forall {Int} {VMInt : VellvmIntegers.VMemInt Int} icmp a b,
       DVCrev.dvalue_convert_strict (@eval_int_icmp Int VMInt icmp a b) =
@@ -8888,174 +9232,6 @@ Qed.
         break_match_goal; inv CONV.
     }
   Qed.
-
-  Lemma fin_to_inf_dvalue_array :
-    forall elts,
-      fin_to_inf_dvalue (DVALUE_Array elts) =
-        DVCrev.DV2.DVALUE_Array (map fin_to_inf_dvalue elts).
-  Proof.
-    induction elts.
-    - cbn.
-      unfold fin_to_inf_dvalue.
-      break_match_goal; clear Heqs; destruct p; clear e0;
-        cbn in e; subst; inv e.
-      auto.
-    - unfold fin_to_inf_dvalue in *.
-      break_match_goal; clear Heqs; destruct p; clear e0;
-        cbn in e; subst; inv e.
-      break_match_hyp_inv.
-      break_match_hyp_inv.
-      break_match_hyp_inv.
-      rewrite map_cons.
-
-      break_match_hyp_inv; clear Heqs; destruct p; clear e0.
-      cbn in e; subst; inv e.
-
-      break_match_hyp_inv.
-      inv Heqo.
-
-      break_match_goal; clear Heqs; destruct p; clear e0.
-      rewrite Heqo0 in e.
-      inv e.
-      auto.
-  Qed.
-
-  Lemma fin_to_inf_dvalue_vector :
-    forall elts,
-      fin_to_inf_dvalue (DVALUE_Vector elts) =
-        DVCrev.DV2.DVALUE_Vector (map fin_to_inf_dvalue elts).
-  Proof.
-    induction elts.
-    - cbn.
-      unfold fin_to_inf_dvalue.
-      break_match_goal; clear Heqs; destruct p; clear e0;
-        cbn in e; subst; inv e.
-      auto.
-    - unfold fin_to_inf_dvalue in *.
-      break_match_goal; clear Heqs; destruct p; clear e0;
-        cbn in e; subst; inv e.
-      break_match_hyp_inv.
-      break_match_hyp_inv.
-      break_match_hyp_inv.
-      rewrite map_cons.
-
-      break_match_hyp_inv; clear Heqs; destruct p; clear e0.
-      cbn in e; subst; inv e.
-
-      break_match_hyp_inv.
-
-      break_match_goal; clear Heqs; destruct p; clear e0.
-      rewrite Heqo0 in e.
-      inv e.
-
-      inv Heqo.
-      auto.
-  Qed.
-
-  Lemma fin_to_inf_dvalue_i1 :
-    forall x,
-      fin_to_inf_dvalue (DVALUE_I1 x) =
-        DVCrev.DV2.DVALUE_I1 x.
-  Proof.
-    intros x.
-    unfold fin_to_inf_dvalue.
-    break_match_goal; clear Heqs; destruct p; clear e0;
-      cbn in e; subst; inv e.
-    auto.
-  Qed.
-
-  Lemma fin_to_inf_dvalue_i8 :
-    forall x,
-      fin_to_inf_dvalue (DVALUE_I8 x) =
-        DVCrev.DV2.DVALUE_I8 x.
-  Proof.
-    intros x.
-    unfold fin_to_inf_dvalue.
-    break_match_goal; clear Heqs; destruct p; clear e0;
-      cbn in e; subst; inv e.
-    auto.
-  Qed.
-
-  Lemma fin_to_inf_dvalue_i32 :
-    forall x,
-      fin_to_inf_dvalue (DVALUE_I32 x) =
-        DVCrev.DV2.DVALUE_I32 x.
-  Proof.
-    intros x.
-    unfold fin_to_inf_dvalue.
-    break_match_goal; clear Heqs; destruct p; clear e0;
-      cbn in e; subst; inv e.
-    auto.
-  Qed.
-
-  Lemma fin_to_inf_dvalue_i64 :
-    forall x,
-      fin_to_inf_dvalue (DVALUE_I64 x) =
-        DVCrev.DV2.DVALUE_I64 x.
-  Proof.
-    intros x.
-    unfold fin_to_inf_dvalue.
-    break_match_goal; clear Heqs; destruct p; clear e0;
-      cbn in e; subst; inv e.
-    auto.
-  Qed.
-
-  Definition intptr_fin_inf (x : IP.intptr) : IS1.LP.IP.intptr.
-    pose proof intptr_convert_succeeds x.
-    destruct H.
-    apply x0.
-  Defined.
-
-  Lemma fin_to_inf_dvalue_iptr :
-    forall x,
-      fin_to_inf_dvalue (DVALUE_IPTR x) =
-        DVCrev.DV2.DVALUE_IPTR (intptr_fin_inf x).
-  Proof.
-    intros x.
-    unfold fin_to_inf_dvalue.
-    break_match_goal; clear Heqs; destruct p; clear e0;
-      cbn in e; subst; inv e.
-
-    pose proof intptr_convert_succeeds x.
-    destruct H.
-    rewrite e in H0.
-    inv H0.
-
-    unfold intptr_fin_inf.
-    break_match_goal.
-    clear Heqs.
-    congruence.
-  Qed.
-
-  Lemma fin_to_inf_dvalue_poison :
-    forall t,
-      fin_to_inf_dvalue (DVALUE_Poison t) =
-        DVCrev.DV2.DVALUE_Poison t.
-  Proof.
-    intros x.
-    unfold fin_to_inf_dvalue.
-    break_match_goal; clear Heqs; destruct p; clear e0;
-      cbn in e; subst; inv e.
-    auto.
-  Qed.
-
-  (* TODO: Move this *)
-  Lemma sizeof_dtyp_fin_inf :
-    forall t,
-      IS1.LP.SIZEOF.sizeof_dtyp t = SIZEOF.sizeof_dtyp t.
-  Proof.
-    (* Need to expose more stuff to be able to prove this *)
-  Admitted.
-
-  Ltac rewrite_fin_to_inf_dvalue :=
-    repeat
-      first
-      [ rewrite fin_to_inf_dvalue_i1
-      | rewrite fin_to_inf_dvalue_i8
-      | rewrite fin_to_inf_dvalue_i32
-      | rewrite fin_to_inf_dvalue_i64
-      | rewrite fin_to_inf_dvalue_iptr
-      ].
 
   Lemma handle_gep_h_fin_inf :
     forall idxs_fin idxs_inf t base res,
@@ -9901,68 +10077,6 @@ Qed.
         reflexivity.
   Qed.
 
-  Lemma fin_to_inf_dvalue_struct :
-    forall elts,
-      fin_to_inf_dvalue (DVALUE_Struct elts) =
-        DVCrev.DV2.DVALUE_Struct (map fin_to_inf_dvalue elts).
-  Proof.
-    induction elts.
-    - cbn.
-      unfold fin_to_inf_dvalue.
-      break_match_goal; clear Heqs; destruct p; clear e0;
-        cbn in e; subst; inv e.
-      auto.
-    - unfold fin_to_inf_dvalue in *.
-      break_match_goal; clear Heqs; destruct p; clear e0;
-        cbn in e; subst; inv e.
-      break_match_hyp_inv.
-      break_match_hyp_inv.
-      break_match_hyp_inv.
-
-      break_match_hyp_inv; clear Heqs; destruct p; clear e0.
-      cbn in e; subst; inv e.
-
-      break_match_hyp_inv.
-      rewrite map_cons.
-      inv Heqo.
-
-      break_match_goal; clear Heqs; destruct p; clear e0.
-      rewrite Heqo0 in e.
-      inv e.
-      auto.
-  Qed.
-
-  Lemma fin_to_inf_dvalue_packed_struct :
-    forall elts,
-      fin_to_inf_dvalue (DVALUE_Packed_struct elts) =
-        DVCrev.DV2.DVALUE_Packed_struct (map fin_to_inf_dvalue elts).
-  Proof.
-    induction elts.
-    - cbn.
-      unfold fin_to_inf_dvalue.
-      break_match_goal; clear Heqs; destruct p; clear e0;
-        cbn in e; subst; inv e.
-      auto.
-    - unfold fin_to_inf_dvalue in *.
-      break_match_goal; clear Heqs; destruct p; clear e0;
-        cbn in e; subst; inv e.
-      break_match_hyp_inv.
-      break_match_hyp_inv.
-      break_match_hyp_inv.
-
-      break_match_hyp_inv; clear Heqs; destruct p; clear e0.
-      cbn in e; subst; inv e.
-
-      break_match_hyp_inv.
-      rewrite map_cons.
-      inv Heqo.
-
-      break_match_goal; clear Heqs; destruct p; clear e0.
-      rewrite Heqo0 in e.
-      inv e.
-      auto.
-  Qed.
-
   Lemma index_into_str_dv_fin_inf :
     forall {v idx} {res : err_ub_oom dvalue},
       index_into_str_dv v idx = res ->
@@ -10672,6 +10786,2087 @@ Qed.
     inv H1.
     auto.
   Qed.
+
+  Lemma uvalue_concretize_strict_concretize_u_inclusion :
+    forall uv_inf uv_fin,
+      uvalue_refine_strict uv_inf uv_fin ->
+      uvalue_concretize_u_fin_inf_inclusion uv_inf uv_fin.
+  Proof.
+    intros uv_inf.
+    induction uv_inf; intros uv_fin REF;
+      try solve
+        [ red; intros dv_fin CONC_FIN;
+          red in REF;
+          cbn in REF; inv REF;
+
+          red in CONC_FIN;
+          rewrite CONCBASE.concretize_uvalueM_equation in CONC_FIN;
+          cbn in CONC_FIN; inversion CONC_FIN; subst;
+
+          red;
+          rewrite IS1.LLVM.MEM.CP.CONCBASE.concretize_uvalueM_equation;
+          cbn;
+          unfold fin_to_inf_dvalue;
+          break_match_goal; clear Heqs; destruct p; clear e0;
+            cbn in e; inv e;
+          reflexivity
+        ].
+    - (* Addresses *)
+      red; intros dv_fin CONC_FIN.
+      red in REF.
+      cbn in REF.
+      break_match_hyp_inv.
+      red in CONC_FIN.
+      rewrite CONCBASE.concretize_uvalueM_equation in CONC_FIN.
+      cbn in CONC_FIN; inv CONC_FIN.
+
+      red.
+      rewrite IS1.LLVM.MEM.CP.CONCBASE.concretize_uvalueM_equation.
+      cbn.
+      unfold fin_to_inf_dvalue.
+      break_match_goal.
+      clear Heqs; destruct p; clear e0.
+      cbn in e.
+      break_match_hyp_inv.
+      pose proof (addr_convert_safe _ _ Heqo0).
+      pose proof (AC1.addr_convert_injective _ _ _ Heqo H0); subst.
+      reflexivity.
+    - (* IPTR *)
+      red; intros dv_fin CONC_FIN.
+      red in REF.
+      cbn in REF.
+      break_match_hyp_inv.
+
+      red.
+      rewrite IS1.LLVM.MEM.CP.CONCBASE.concretize_uvalueM_equation.
+      cbn.
+      unfold fin_to_inf_dvalue.
+      cbn in CONC_FIN; subst.
+      cbn.
+      break_match_goal.
+      cbn in *.
+      clear Heqs; destruct p; clear e0.
+      cbn in e.
+      break_match_hyp_inv.
+      pose proof (intptr_convert_safe _ _ Heqo0).
+      pose proof IP.from_Z_injective _ _ _ Heqo H.
+      apply IS1.LP.IP.to_Z_inj in H0; subst.
+      reflexivity.
+    - (* Undef *)
+      red; intros dv_fin CONC_FIN.
+      red in REF.
+      cbn in REF; inv REF.
+
+      red in CONC_FIN.
+      rewrite CONCBASE.concretize_uvalueM_equation in CONC_FIN.
+      cbn in CONC_FIN.
+
+      red.
+      rewrite IS1.LLVM.MEM.CP.CONCBASE.concretize_uvalueM_equation.
+      cbn.
+
+      repeat break_match_hyp; try contradiction.
+      destruct CONC_FIN.
+      split.
+      eapply dvalue_has_dtyp_fin_to_inf_dvalue; eauto.
+      eapply fin_to_inf_dvalue_not_poison; auto.
+
+    - (* Struct *)
+      red; intros dv_fin CONC_FIN.
+      red in REF.
+      cbn in REF.
+      break_match_hyp_inv.
+
+      unfold uvalue_concretize_fin_inf_inclusion in H.
+      apply map_monad_oom_Forall2 in Heqo.
+
+      red.
+      rewrite IS1.LLVM.MEM.CP.CONCBASE.concretize_uvalueM_equation.
+
+      red in CONC_FIN.
+      rewrite IS2.LLVM.MEM.CP.CONCBASE.concretize_uvalueM_equation in CONC_FIN.
+
+      repeat red in CONC_FIN.
+      destruct CONC_FIN as (?&?&?&?&?).
+
+      destruct_err_ub_oom x; cbn in H1; inv H1.
+      { (* OOM *)
+        clear H2 H3.
+        (* TODO: Can this be refactored into a more general lemma? *)
+        induction Heqo.
+        - cbn in *.
+          inv H0.
+        - rewrite map_monad_unfold.
+          rewrite map_monad_unfold in H0.
+          repeat red in H0.
+          destruct H0 as (?&?&?&?&?).
+          repeat red.
+
+          pose proof H0.
+          eapply H in H4.
+          2: left; eauto.
+          all: eauto.
+
+          destruct_err_ub_oom x1; cbn in H2; inv H2.
+          { cbn in H4.
+            exists (OOM_unERR_UB_OOM oom_x).
+            eexists.
+            red in H4.
+            cbn.
+            unfold bind_ErrUbOomProp.
+            split; eauto.
+            exists (OOM_unERR_UB_OOM oom_x).
+            eexists.
+            split; cbn; eauto.
+          }
+
+          destruct H3 as [[] | H3].
+          specialize (H3 x3).
+          forward H3. reflexivity.
+          cbn in H3.
+          red in H3.
+          destruct H3 as (?&?&?&?&?).
+
+          destruct_err_ub_oom x1; cbn in H3; rewrite <- H3 in H6; inv H6.
+          { cbn in H4.
+            exists (OOM_unERR_UB_OOM oom_x).
+            exists (fun _ => (OOM_unERR_UB_OOM oom_x)).
+            cbn.
+            unfold bind_ErrUbOomProp.
+            split.
+            - exists (success_unERR_UB_OOM (fin_to_inf_dvalue x3)).
+              exists (fun _ => (OOM_unERR_UB_OOM oom_x)).
+              split; cbn; eauto.
+              split; cbn; eauto.
+              right.
+              intros a H6.
+              exists (OOM_unERR_UB_OOM oom_x).
+              exists (fun _ => (OOM_unERR_UB_OOM oom_x)).
+              cbn.
+              split; cbn; eauto.
+              forward IHHeqo.
+              intros u H7 uv_fin H8; eapply H; eauto; right; eauto.
+              subst.
+              forward IHHeqo; eauto.
+              cbn in IHHeqo.
+              unfold bind_ErrUbOomProp in IHHeqo.
+              destruct IHHeqo as (?&?&?&?&?).
+
+              destruct_err_ub_oom x1; subst; cbn in H7; inv H7; auto.
+
+              destruct H8 as [[] | H8].
+              specialize (H8 x6 eq_refl).
+              rewrite <- H8 in H10; inv H10.
+            - split; eauto.
+          }
+
+          cbn in H4.
+          destruct H5 as [[] | H5].
+          specialize (H5 _ eq_refl).
+          rewrite <- H5 in H8.
+          inv H8.
+      }
+
+      { (* UB *)
+        clear H2 H3.
+        (* TODO: Can this be refactored into a more general lemma? *)
+        induction Heqo.
+        - cbn in *.
+          inv H0.
+        - rewrite map_monad_unfold.
+          rewrite map_monad_unfold in H0.
+          repeat red in H0.
+          destruct H0 as (?&?&?&?&?).
+          repeat red.
+
+          pose proof H0.
+          eapply H in H4.
+          2: left; eauto.
+          all: eauto.
+
+          destruct_err_ub_oom x1; cbn in H2; inv H2.
+          { cbn in H4.
+            exists (UB_unERR_UB_OOM ub_x).
+            eexists.
+            red in H4.
+            cbn.
+            unfold bind_ErrUbOomProp.
+            split; eauto.
+            exists (UB_unERR_UB_OOM ub_x).
+            eexists.
+            split; cbn; eauto.
+          }
+
+          destruct H3 as [[] | H3].
+          specialize (H3 x3).
+          forward H3. reflexivity.
+          cbn in H3.
+          red in H3.
+          destruct H3 as (?&?&?&?&?).
+
+          destruct_err_ub_oom x1; cbn in H3; rewrite <- H3 in H6; inv H6.
+          { cbn in H4.
+            exists (UB_unERR_UB_OOM ub_x).
+            exists (fun _ => (UB_unERR_UB_OOM ub_x)).
+            cbn.
+            unfold bind_ErrUbOomProp.
+            split.
+            - exists (success_unERR_UB_OOM (fin_to_inf_dvalue x3)).
+              exists (fun _ => (UB_unERR_UB_OOM ub_x)).
+              split; cbn; eauto.
+              split; cbn; eauto.
+              right.
+              intros a H6.
+              exists (UB_unERR_UB_OOM ub_x).
+              exists (fun _ => (UB_unERR_UB_OOM ub_x)).
+              cbn.
+              split; cbn; eauto.
+              forward IHHeqo.
+              intros u H7 uv_fin H8; eapply H; eauto; right; eauto.
+              subst.
+              forward IHHeqo; eauto.
+              cbn in IHHeqo.
+              unfold bind_ErrUbOomProp in IHHeqo.
+              destruct IHHeqo as (?&?&?&?&?).
+
+              destruct_err_ub_oom x1; subst; cbn in H7; inv H7; auto.
+
+              destruct H8 as [[] | H8].
+              specialize (H8 x6 eq_refl).
+              rewrite <- H8 in H10; inv H10.
+            - split; eauto.
+          }
+
+          cbn in H4.
+          destruct H5 as [[] | H5].
+          specialize (H5 _ eq_refl).
+          rewrite <- H5 in H8.
+          inv H8.
+      }
+
+      { (* Err *)
+        clear H2 H3.
+        (* TODO: Can this be refactored into a more general lemma? *)
+        induction Heqo.
+        - cbn in *.
+          inv H0.
+        - rewrite map_monad_unfold.
+          rewrite map_monad_unfold in H0.
+          repeat red in H0.
+          destruct H0 as (?&?&?&?&?).
+          repeat red.
+
+          pose proof H0.
+          eapply H in H4.
+          2: left; eauto.
+          all: eauto.
+
+          destruct_err_ub_oom x1; cbn in H2; inv H2.
+          { cbn in H4.
+            exists (ERR_unERR_UB_OOM err_x).
+            eexists.
+            red in H4.
+            cbn.
+            unfold bind_ErrUbOomProp.
+            split; eauto.
+            exists (ERR_unERR_UB_OOM err_x).
+            eexists.
+            split; cbn; eauto.
+          }
+
+          destruct H3 as [[] | H3].
+          specialize (H3 x3).
+          forward H3. reflexivity.
+          cbn in H3.
+          red in H3.
+          destruct H3 as (?&?&?&?&?).
+
+          destruct_err_ub_oom x1; cbn in H3; rewrite <- H3 in H6; inv H6.
+          { cbn in H4.
+            exists (ERR_unERR_UB_OOM err_x).
+            exists (fun _ => (ERR_unERR_UB_OOM err_x)).
+            cbn.
+            unfold bind_ErrUbOomProp.
+            split.
+            - exists (success_unERR_UB_OOM (fin_to_inf_dvalue x3)).
+              exists (fun _ => (ERR_unERR_UB_OOM err_x)).
+              split; cbn; eauto.
+              split; cbn; eauto.
+              right.
+              intros a H6.
+              exists (ERR_unERR_UB_OOM err_x).
+              exists (fun _ => (ERR_unERR_UB_OOM err_x)).
+              cbn.
+              split; cbn; eauto.
+              forward IHHeqo.
+              intros u H7 uv_fin H8; eapply H; eauto; right; eauto.
+              subst.
+              forward IHHeqo; eauto.
+              cbn in IHHeqo.
+              unfold bind_ErrUbOomProp in IHHeqo.
+              destruct IHHeqo as (?&?&?&?&?).
+
+              destruct_err_ub_oom x1; subst; cbn in H7; inv H7; auto.
+
+              destruct H8 as [[] | H8].
+              specialize (H8 x6 eq_refl).
+              rewrite <- H8 in H10; inv H10.
+            - split; eauto.
+          }
+
+          cbn in H4.
+          destruct H5 as [[] | H5].
+          specialize (H5 _ eq_refl).
+          rewrite <- H5 in H8.
+          inv H8.
+      }
+
+      destruct H2 as [[] | H2].
+      specialize (H2 x1 eq_refl).
+      cbn in H2.
+      rewrite <- H2 in H3.
+      cbn in H3. inv H3.
+      rewrite <- H2.
+
+      rename H0 into MAP.
+
+      repeat red.
+      exists (ret (map fin_to_inf_dvalue x1)).
+      exists (fun fields => ret (IS1.LP.Events.DV.DVALUE_Struct fields)).
+      split.
+      { eapply map_monad_ErrUbOomProp_forall2.
+        apply Util.Forall2_forall.
+        split.
+        - rewrite map_length.
+
+          apply map_monad_ErrUbOomProp_length in MAP.
+          apply Util.Forall2_length in Heqo.
+          congruence.
+        - intros i a b NTH_fields NTH_res.
+
+          epose proof Util.Forall2_Nth_left NTH_fields Heqo as (x&NTHl&CONV).
+
+          apply Util.Nth_In in NTH_fields.
+          specialize (H a NTH_fields x CONV).
+
+          eapply map_monad_ErrUbOomProp_forall2 in MAP.
+          epose proof Util.Forall2_Nth_left NTHl MAP as (?&NTH_CONC&CONC).
+          specialize (H _ CONC).
+
+          apply Nth_map_iff in NTH_res as (?&?&?).
+          subst.
+
+          red in NTH_CONC, H1.
+          rewrite H1 in NTH_CONC.
+          inv NTH_CONC.
+          apply H.
+      }
+
+      cbn.
+      split.
+      { unfold fin_to_inf_dvalue at 2.
+        break_match_goal.
+        clear Heqs; destruct p; clear e0.
+
+        erewrite <- dvalue_convert_strict_struct_map; eauto.
+      }
+
+      right.
+      intros a H0.
+      reflexivity.
+    - (* Packed structs *)
+      red; intros dv_fin CONC_FIN.
+      red in REF.
+      cbn in REF.
+      break_match_hyp_inv.
+
+      unfold uvalue_concretize_fin_inf_inclusion in H.
+      apply map_monad_oom_Forall2 in Heqo.
+
+      red.
+      rewrite IS1.LLVM.MEM.CP.CONCBASE.concretize_uvalueM_equation.
+
+      red in CONC_FIN.
+      rewrite IS2.LLVM.MEM.CP.CONCBASE.concretize_uvalueM_equation in CONC_FIN.
+
+      repeat red in CONC_FIN.
+      destruct CONC_FIN as (?&?&?&?&?).
+
+      destruct_err_ub_oom x; cbn in H1; inv H1.
+      { (* OOM *)
+        clear H2 H3.
+        (* TODO: Can this be refactored into a more general lemma? *)
+        induction Heqo.
+        - cbn in *.
+          inv H0.
+        - rewrite map_monad_unfold.
+          rewrite map_monad_unfold in H0.
+          repeat red in H0.
+          destruct H0 as (?&?&?&?&?).
+          repeat red.
+
+          pose proof H0.
+          eapply H in H4.
+          2: left; eauto.
+          all: eauto.
+
+          destruct_err_ub_oom x1; cbn in H2; inv H2.
+          { cbn in H4.
+            exists (OOM_unERR_UB_OOM oom_x).
+            eexists.
+            red in H4.
+            cbn.
+            unfold bind_ErrUbOomProp.
+            split; eauto.
+            exists (OOM_unERR_UB_OOM oom_x).
+            eexists.
+            split; cbn; eauto.
+          }
+
+          destruct H3 as [[] | H3].
+          specialize (H3 x3).
+          forward H3. reflexivity.
+          cbn in H3.
+          red in H3.
+          destruct H3 as (?&?&?&?&?).
+
+          destruct_err_ub_oom x1; cbn in H3; rewrite <- H3 in H6; inv H6.
+          { cbn in H4.
+            exists (OOM_unERR_UB_OOM oom_x).
+            exists (fun _ => (OOM_unERR_UB_OOM oom_x)).
+            cbn.
+            unfold bind_ErrUbOomProp.
+            split.
+            - exists (success_unERR_UB_OOM (fin_to_inf_dvalue x3)).
+              exists (fun _ => (OOM_unERR_UB_OOM oom_x)).
+              split; cbn; eauto.
+              split; cbn; eauto.
+              right.
+              intros a H6.
+              exists (OOM_unERR_UB_OOM oom_x).
+              exists (fun _ => (OOM_unERR_UB_OOM oom_x)).
+              cbn.
+              split; cbn; eauto.
+              forward IHHeqo.
+              intros u H7 uv_fin H8; eapply H; eauto; right; eauto.
+              subst.
+              forward IHHeqo; eauto.
+              cbn in IHHeqo.
+              unfold bind_ErrUbOomProp in IHHeqo.
+              destruct IHHeqo as (?&?&?&?&?).
+
+              destruct_err_ub_oom x1; subst; cbn in H7; inv H7; auto.
+
+              destruct H8 as [[] | H8].
+              specialize (H8 x6 eq_refl).
+              rewrite <- H8 in H10; inv H10.
+            - split; eauto.
+          }
+
+          cbn in H4.
+          destruct H5 as [[] | H5].
+          specialize (H5 _ eq_refl).
+          rewrite <- H5 in H8.
+          inv H8.
+      }
+
+      { (* UB *)
+        clear H2 H3.
+        (* TODO: Can this be refactored into a more general lemma? *)
+        induction Heqo.
+        - cbn in *.
+          inv H0.
+        - rewrite map_monad_unfold.
+          rewrite map_monad_unfold in H0.
+          repeat red in H0.
+          destruct H0 as (?&?&?&?&?).
+          repeat red.
+
+          pose proof H0.
+          eapply H in H4.
+          2: left; eauto.
+          all: eauto.
+
+          destruct_err_ub_oom x1; cbn in H2; inv H2.
+          { cbn in H4.
+            exists (UB_unERR_UB_OOM ub_x).
+            eexists.
+            red in H4.
+            cbn.
+            unfold bind_ErrUbOomProp.
+            split; eauto.
+            exists (UB_unERR_UB_OOM ub_x).
+            eexists.
+            split; cbn; eauto.
+          }
+
+          destruct H3 as [[] | H3].
+          specialize (H3 x3).
+          forward H3. reflexivity.
+          cbn in H3.
+          red in H3.
+          destruct H3 as (?&?&?&?&?).
+
+          destruct_err_ub_oom x1; cbn in H3; rewrite <- H3 in H6; inv H6.
+          { cbn in H4.
+            exists (UB_unERR_UB_OOM ub_x).
+            exists (fun _ => (UB_unERR_UB_OOM ub_x)).
+            cbn.
+            unfold bind_ErrUbOomProp.
+            split.
+            - exists (success_unERR_UB_OOM (fin_to_inf_dvalue x3)).
+              exists (fun _ => (UB_unERR_UB_OOM ub_x)).
+              split; cbn; eauto.
+              split; cbn; eauto.
+              right.
+              intros a H6.
+              exists (UB_unERR_UB_OOM ub_x).
+              exists (fun _ => (UB_unERR_UB_OOM ub_x)).
+              cbn.
+              split; cbn; eauto.
+              forward IHHeqo.
+              intros u H7 uv_fin H8; eapply H; eauto; right; eauto.
+              subst.
+              forward IHHeqo; eauto.
+              cbn in IHHeqo.
+              unfold bind_ErrUbOomProp in IHHeqo.
+              destruct IHHeqo as (?&?&?&?&?).
+
+              destruct_err_ub_oom x1; subst; cbn in H7; inv H7; auto.
+
+              destruct H8 as [[] | H8].
+              specialize (H8 x6 eq_refl).
+              rewrite <- H8 in H10; inv H10.
+            - split; eauto.
+          }
+
+          cbn in H4.
+          destruct H5 as [[] | H5].
+          specialize (H5 _ eq_refl).
+          rewrite <- H5 in H8.
+          inv H8.
+      }
+
+      { (* Err *)
+        clear H2 H3.
+        (* TODO: Can this be refactored into a more general lemma? *)
+        induction Heqo.
+        - cbn in *.
+          inv H0.
+        - rewrite map_monad_unfold.
+          rewrite map_monad_unfold in H0.
+          repeat red in H0.
+          destruct H0 as (?&?&?&?&?).
+          repeat red.
+
+          pose proof H0.
+          eapply H in H4.
+          2: left; eauto.
+          all: eauto.
+
+          destruct_err_ub_oom x1; cbn in H2; inv H2.
+          { cbn in H4.
+            exists (ERR_unERR_UB_OOM err_x).
+            eexists.
+            red in H4.
+            cbn.
+            unfold bind_ErrUbOomProp.
+            split; eauto.
+            exists (ERR_unERR_UB_OOM err_x).
+            eexists.
+            split; cbn; eauto.
+          }
+
+          destruct H3 as [[] | H3].
+          specialize (H3 x3).
+          forward H3. reflexivity.
+          cbn in H3.
+          red in H3.
+          destruct H3 as (?&?&?&?&?).
+
+          destruct_err_ub_oom x1; cbn in H3; rewrite <- H3 in H6; inv H6.
+          { cbn in H4.
+            exists (ERR_unERR_UB_OOM err_x).
+            exists (fun _ => (ERR_unERR_UB_OOM err_x)).
+            cbn.
+            unfold bind_ErrUbOomProp.
+            split.
+            - exists (success_unERR_UB_OOM (fin_to_inf_dvalue x3)).
+              exists (fun _ => (ERR_unERR_UB_OOM err_x)).
+              split; cbn; eauto.
+              split; cbn; eauto.
+              right.
+              intros a H6.
+              exists (ERR_unERR_UB_OOM err_x).
+              exists (fun _ => (ERR_unERR_UB_OOM err_x)).
+              cbn.
+              split; cbn; eauto.
+              forward IHHeqo.
+              intros u H7 uv_fin H8; eapply H; eauto; right; eauto.
+              subst.
+              forward IHHeqo; eauto.
+              cbn in IHHeqo.
+              unfold bind_ErrUbOomProp in IHHeqo.
+              destruct IHHeqo as (?&?&?&?&?).
+
+              destruct_err_ub_oom x1; subst; cbn in H7; inv H7; auto.
+
+              destruct H8 as [[] | H8].
+              specialize (H8 x6 eq_refl).
+              rewrite <- H8 in H10; inv H10.
+            - split; eauto.
+          }
+
+          cbn in H4.
+          destruct H5 as [[] | H5].
+          specialize (H5 _ eq_refl).
+          rewrite <- H5 in H8.
+          inv H8.
+      }
+
+      destruct H2 as [[] | H2].
+      specialize (H2 x1 eq_refl).
+      cbn in H2.
+      rewrite <- H2 in H3.
+      cbn in H3. inv H3.
+      rewrite <- H2.
+
+      rename H0 into MAP.
+
+      repeat red.
+      exists (ret (map fin_to_inf_dvalue x1)).
+      exists (fun fields => ret (IS1.LP.Events.DV.DVALUE_Packed_struct fields)).
+      split.
+      { eapply map_monad_ErrUbOomProp_forall2.
+        apply Util.Forall2_forall.
+        split.
+        - rewrite map_length.
+
+          apply map_monad_ErrUbOomProp_length in MAP.
+          apply Util.Forall2_length in Heqo.
+          congruence.
+        - intros i a b NTH_fields NTH_res.
+
+          epose proof Util.Forall2_Nth_left NTH_fields Heqo as (x&NTHl&CONV).
+
+          apply Util.Nth_In in NTH_fields.
+          specialize (H a NTH_fields x CONV).
+
+          eapply map_monad_ErrUbOomProp_forall2 in MAP.
+          epose proof Util.Forall2_Nth_left NTHl MAP as (?&NTH_CONC&CONC).
+          specialize (H _ CONC).
+
+          apply Nth_map_iff in NTH_res as (?&?&?).
+          subst.
+
+          red in NTH_CONC, H1.
+          rewrite H1 in NTH_CONC.
+          inv NTH_CONC.
+          apply H.
+      }
+
+      cbn.
+      split.
+      { unfold fin_to_inf_dvalue at 2.
+        break_match_goal.
+        clear Heqs; destruct p; clear e0.
+
+        erewrite <- dvalue_convert_strict_packed_struct_map; eauto.
+      }
+
+      right.
+      intros a H0.
+      reflexivity.
+    - (* Array *)
+      red; intros dv_fin CONC_FIN.
+      red in REF.
+      cbn in REF.
+      break_match_hyp_inv.
+
+      unfold uvalue_concretize_u_fin_inf_inclusion in H.
+      apply map_monad_oom_Forall2 in Heqo.
+
+      red.
+      rewrite IS1.LLVM.MEM.CP.CONCBASE.concretize_uvalueM_equation.
+
+      red in CONC_FIN.
+      rewrite IS2.LLVM.MEM.CP.CONCBASE.concretize_uvalueM_equation in CONC_FIN.
+
+      revert dv_fin CONC_FIN.
+
+      induction Heqo; intros dv_fin CONC_FIN;
+        repeat red in CONC_FIN;
+        destruct CONC_FIN as (?&?&?&?&?).      
+      + cbn in H0.
+        inv H0.
+        destruct H2 as [[] | H2].
+
+        specialize (H2 _ eq_refl).
+        cbn in H2.
+
+        repeat red.
+        exists (success_unERR_UB_OOM []).
+        exists (fun _ => success_unERR_UB_OOM (fin_to_inf_dvalue (DVALUE_Array []))).
+        split; cbn; eauto.
+        rewrite <- H2.
+        cbn.
+        split; eauto.
+        right.
+        intros; subst.
+        rewrite fin_to_inf_dvalue_array.
+        cbn.
+        auto.
+      + forward IHHeqo.
+        { intros e H4 uv_fin H5 res H6.
+          eapply H.
+          right; auto.
+          apply H5.
+          auto.
+        }
+
+        rewrite map_monad_unfold in H1.
+        repeat red in H1.
+        destruct H1 as (?&?&?&?&?).
+        subst.
+
+        pose proof (H x (or_introl eq_refl) _ H0 _ H1).
+        destruct_err_ub_oom x2; subst.
+
+        { (* OOM *)
+          clear H5 H3.
+          exists (OOM_unERR_UB_OOM oom_x).
+          eexists.
+          split; cbn; eauto.
+
+          red.
+          exists (fmap fin_to_inf_dvalue (OOM_unERR_UB_OOM oom_x)).
+          eexists.
+          split; cbn; eauto.
+        }
+
+        { (* UB *)
+          clear H5 H3.
+          exists (UB_unERR_UB_OOM ub_x).
+          eexists.
+          split; cbn; eauto.
+
+          red.
+          exists (fmap fin_to_inf_dvalue (UB_unERR_UB_OOM ub_x)).
+          eexists.
+          split; cbn; eauto.
+        }
+
+        { (* Err *)
+          clear H5 H3.
+          exists (ERR_unERR_UB_OOM err_x).
+          eexists.
+          split; cbn; eauto.
+
+          red.
+          exists (fmap fin_to_inf_dvalue (ERR_unERR_UB_OOM err_x)).
+          eexists.
+          split; cbn; eauto.
+        }
+
+        destruct H5 as [[] | H5].
+        specialize (H5 _ eq_refl).
+        repeat red in H5.
+        destruct H5 as (?&?&?&?&?).
+
+        destruct_err_ub_oom x2; cbn in H5, H3; rewrite <- H5 in H3; cbn in H3; subst.
+        { (* OOM *)
+          clear H3 H6.
+          cbn; setoid_rewrite <- H5.
+          exists (OOM_unERR_UB_OOM oom_x).
+          eexists.
+          split; cbn; eauto.
+
+          red.
+          exists (fmap fin_to_inf_dvalue (success_unERR_UB_OOM x0)).
+          exists (fun _ => OOM_unERR_UB_OOM oom_x).
+          split; cbn; eauto.
+          split; cbn; eauto.
+          right.
+          intros; subst.
+          red.
+
+          exists (OOM_unERR_UB_OOM oom_x).
+          eexists.
+          split; cbn; eauto.
+
+          specialize (IHHeqo (OOM_unERR_UB_OOM oom_x)).
+          forward IHHeqo.
+          { cbn.
+            red.
+            exists (OOM_unERR_UB_OOM oom_x).
+            eexists.
+            split; cbn; eauto.
+          }
+
+          repeat red in IHHeqo.
+          destruct IHHeqo as (?&?&?&?&?).
+          destruct_err_ub_oom x2; cbn in H6; inv H6; eauto.
+
+          destruct H7 as [[] | H7].
+          specialize (H7 _ eq_refl).
+          cbn in H7.
+          rewrite <- H7 in H9.
+          cbn in H9.
+          inv H9.
+        }
+
+        { (* UB *)
+          clear H3 H6.
+          cbn; setoid_rewrite <- H5.
+          exists (UB_unERR_UB_OOM ub_x).
+          eexists.
+          split; cbn; eauto.
+
+          red.
+          exists (fmap fin_to_inf_dvalue (success_unERR_UB_OOM x0)).
+          exists (fun _ => UB_unERR_UB_OOM ub_x).
+          split; cbn; eauto.
+          split; cbn; eauto.
+          right.
+          intros; subst.
+          red.
+
+          exists (UB_unERR_UB_OOM ub_x).
+          eexists.
+          split; cbn; eauto.
+
+          specialize (IHHeqo (UB_unERR_UB_OOM ub_x)).
+          forward IHHeqo.
+          { cbn.
+            red.
+            exists (UB_unERR_UB_OOM ub_x).
+            eexists.
+            split; cbn; eauto.
+          }
+
+          repeat red in IHHeqo.
+          destruct IHHeqo as (?&?&?&?&?).
+          destruct_err_ub_oom x2; cbn in H6; inv H6; eauto.
+
+          destruct H7 as [[] | H7].
+          specialize (H7 _ eq_refl).
+          cbn in H7.
+          rewrite <- H7 in H9.
+          cbn in H9.
+          inv H9.
+        }
+
+        { (* Err *)
+          clear H3 H6.
+          cbn; setoid_rewrite <- H5.
+          exists (ERR_unERR_UB_OOM err_x).
+          eexists.
+          split; cbn; eauto.
+
+          red.
+          exists (fmap fin_to_inf_dvalue (success_unERR_UB_OOM x0)).
+          exists (fun _ => ERR_unERR_UB_OOM err_x).
+          split; cbn; eauto.
+          split; cbn; eauto.
+          right.
+          intros; subst.
+          red.
+
+          exists (ERR_unERR_UB_OOM err_x).
+          eexists.
+          split; cbn; eauto.
+
+          specialize (IHHeqo (ERR_unERR_UB_OOM err_x)).
+          forward IHHeqo.
+          { cbn.
+            red.
+            exists (ERR_unERR_UB_OOM err_x).
+            eexists.
+            split; cbn; eauto.
+          }
+
+          repeat red in IHHeqo.
+          destruct IHHeqo as (?&?&?&?&?).
+          destruct_err_ub_oom x2; cbn in H6; inv H6; eauto.
+
+          destruct H7 as [[] | H7].
+          specialize (H7 _ eq_refl).
+          cbn in H7.
+          rewrite <- H7 in H9.
+          cbn in H9.
+          inv H9.
+        }
+
+        destruct H6 as [[] | H6].
+        specialize (H6 _ eq_refl).
+        cbn in H6.
+        rewrite <- H6 in H3.
+        cbn in H3.
+        destruct H3 as [[] | H3].
+        specialize (H3 _ eq_refl).
+
+        specialize (IHHeqo (success_unERR_UB_OOM (DVALUE_Array x5))).
+        forward IHHeqo.
+        { cbn.
+          red.
+          exists (success_unERR_UB_OOM x5).
+          exists (fun xs => ret (DVALUE_Array xs)).
+          split; cbn; eauto.
+        }
+
+        repeat red in IHHeqo.
+        destruct IHHeqo as (?&?&?&?&?).
+        destruct_err_ub_oom x2; cbn in H8; inv H8.
+        destruct H9 as [[] | H9].
+        specialize (H9 _ eq_refl).
+        cbn in H9.
+        rewrite <- H9 in H11.
+        inv H11.
+        rewrite <- H6 in H5.
+        inv H5.
+
+        repeat red.
+        exists (ret (fmap fin_to_inf_dvalue (x0::x5))).
+        exists (fun xs => ret (IS1.LP.Events.DV.DVALUE_Array xs)).
+        rewrite map_monad_unfold.
+        split; cbn; eauto.
+        2: {
+          rewrite <- H11; cbn.
+          rewrite <- H3; cbn.
+          split; cbn; eauto.
+          rewrite fin_to_inf_dvalue_array.
+          cbn.
+          reflexivity.
+        }
+
+        exists (fmap fin_to_inf_dvalue (success_unERR_UB_OOM x0)).
+        exists (fun _ => ret (fmap fin_to_inf_dvalue (x0 :: x5))).
+        split; cbn; eauto.
+        split; cbn; eauto.
+        right.
+        intros; subst.
+        red.
+
+        exists (success_unERR_UB_OOM x7).
+        exists (fun _ => ret (fmap fin_to_inf_dvalue (x0 :: x5))).
+        split; cbn; eauto.
+        split; cbn; eauto.
+        right.
+        intros; subst.
+        rewrite fin_to_inf_dvalue_array in H10.
+        inv H10.
+        { (* TODO: should probably make this a lemma... *)
+          induction x5; eauto.
+        }
+    - (* Vector *)
+      red; intros dv_fin CONC_FIN.
+      red in REF.
+      cbn in REF.
+      break_match_hyp_inv.
+
+      unfold uvalue_concretize_u_fin_inf_inclusion in H.
+      apply map_monad_oom_Forall2 in Heqo.
+
+      red.
+      rewrite IS1.LLVM.MEM.CP.CONCBASE.concretize_uvalueM_equation.
+
+      red in CONC_FIN.
+      rewrite IS2.LLVM.MEM.CP.CONCBASE.concretize_uvalueM_equation in CONC_FIN.
+
+      revert dv_fin CONC_FIN.
+
+      induction Heqo; intros dv_fin CONC_FIN;
+        repeat red in CONC_FIN;
+        destruct CONC_FIN as (?&?&?&?&?).      
+      + cbn in H0.
+        inv H0.
+        destruct H2 as [[] | H2].
+
+        specialize (H2 _ eq_refl).
+        cbn in H2.
+
+        repeat red.
+        exists (success_unERR_UB_OOM []).
+        exists (fun _ => success_unERR_UB_OOM (fin_to_inf_dvalue (DVALUE_Vector []))).
+        split; cbn; eauto.
+        rewrite <- H2.
+        cbn.
+        split; eauto.
+        right.
+        intros; subst.
+        rewrite fin_to_inf_dvalue_vector.
+        cbn.
+        auto.
+      + forward IHHeqo.
+        { intros e H4 uv_fin H5 res H6.
+          eapply H.
+          right; auto.
+          apply H5.
+          auto.
+        }
+
+        rewrite map_monad_unfold in H1.
+        repeat red in H1.
+        destruct H1 as (?&?&?&?&?).
+        subst.
+
+        pose proof (H x (or_introl eq_refl) _ H0 _ H1).
+        destruct_err_ub_oom x2; subst.
+
+        { (* OOM *)
+          clear H5 H3.
+          exists (OOM_unERR_UB_OOM oom_x).
+          eexists.
+          split; cbn; eauto.
+
+          red.
+          exists (fmap fin_to_inf_dvalue (OOM_unERR_UB_OOM oom_x)).
+          eexists.
+          split; cbn; eauto.
+        }
+
+        { (* UB *)
+          clear H5 H3.
+          exists (UB_unERR_UB_OOM ub_x).
+          eexists.
+          split; cbn; eauto.
+
+          red.
+          exists (fmap fin_to_inf_dvalue (UB_unERR_UB_OOM ub_x)).
+          eexists.
+          split; cbn; eauto.
+        }
+
+        { (* Err *)
+          clear H5 H3.
+          exists (ERR_unERR_UB_OOM err_x).
+          eexists.
+          split; cbn; eauto.
+
+          red.
+          exists (fmap fin_to_inf_dvalue (ERR_unERR_UB_OOM err_x)).
+          eexists.
+          split; cbn; eauto.
+        }
+
+        destruct H5 as [[] | H5].
+        specialize (H5 _ eq_refl).
+        repeat red in H5.
+        destruct H5 as (?&?&?&?&?).
+
+        destruct_err_ub_oom x2; cbn in H5, H3; rewrite <- H5 in H3; cbn in H3; subst.
+        { (* OOM *)
+          clear H3 H6.
+          cbn; setoid_rewrite <- H5.
+          exists (OOM_unERR_UB_OOM oom_x).
+          eexists.
+          split; cbn; eauto.
+
+          red.
+          exists (fmap fin_to_inf_dvalue (success_unERR_UB_OOM x0)).
+          exists (fun _ => OOM_unERR_UB_OOM oom_x).
+          split; cbn; eauto.
+          split; cbn; eauto.
+          right.
+          intros; subst.
+          red.
+
+          exists (OOM_unERR_UB_OOM oom_x).
+          eexists.
+          split; cbn; eauto.
+
+          specialize (IHHeqo (OOM_unERR_UB_OOM oom_x)).
+          forward IHHeqo.
+          { cbn.
+            red.
+            exists (OOM_unERR_UB_OOM oom_x).
+            eexists.
+            split; cbn; eauto.
+          }
+
+          repeat red in IHHeqo.
+          destruct IHHeqo as (?&?&?&?&?).
+          destruct_err_ub_oom x2; cbn in H6; inv H6; eauto.
+
+          destruct H7 as [[] | H7].
+          specialize (H7 _ eq_refl).
+          cbn in H7.
+          rewrite <- H7 in H9.
+          cbn in H9.
+          inv H9.
+        }
+
+        { (* UB *)
+          clear H3 H6.
+          cbn; setoid_rewrite <- H5.
+          exists (UB_unERR_UB_OOM ub_x).
+          eexists.
+          split; cbn; eauto.
+
+          red.
+          exists (fmap fin_to_inf_dvalue (success_unERR_UB_OOM x0)).
+          exists (fun _ => UB_unERR_UB_OOM ub_x).
+          split; cbn; eauto.
+          split; cbn; eauto.
+          right.
+          intros; subst.
+          red.
+
+          exists (UB_unERR_UB_OOM ub_x).
+          eexists.
+          split; cbn; eauto.
+
+          specialize (IHHeqo (UB_unERR_UB_OOM ub_x)).
+          forward IHHeqo.
+          { cbn.
+            red.
+            exists (UB_unERR_UB_OOM ub_x).
+            eexists.
+            split; cbn; eauto.
+          }
+
+          repeat red in IHHeqo.
+          destruct IHHeqo as (?&?&?&?&?).
+          destruct_err_ub_oom x2; cbn in H6; inv H6; eauto.
+
+          destruct H7 as [[] | H7].
+          specialize (H7 _ eq_refl).
+          cbn in H7.
+          rewrite <- H7 in H9.
+          cbn in H9.
+          inv H9.
+        }
+
+        { (* Err *)
+          clear H3 H6.
+          cbn; setoid_rewrite <- H5.
+          exists (ERR_unERR_UB_OOM err_x).
+          eexists.
+          split; cbn; eauto.
+
+          red.
+          exists (fmap fin_to_inf_dvalue (success_unERR_UB_OOM x0)).
+          exists (fun _ => ERR_unERR_UB_OOM err_x).
+          split; cbn; eauto.
+          split; cbn; eauto.
+          right.
+          intros; subst.
+          red.
+
+          exists (ERR_unERR_UB_OOM err_x).
+          eexists.
+          split; cbn; eauto.
+
+          specialize (IHHeqo (ERR_unERR_UB_OOM err_x)).
+          forward IHHeqo.
+          { cbn.
+            red.
+            exists (ERR_unERR_UB_OOM err_x).
+            eexists.
+            split; cbn; eauto.
+          }
+
+          repeat red in IHHeqo.
+          destruct IHHeqo as (?&?&?&?&?).
+          destruct_err_ub_oom x2; cbn in H6; inv H6; eauto.
+
+          destruct H7 as [[] | H7].
+          specialize (H7 _ eq_refl).
+          cbn in H7.
+          rewrite <- H7 in H9.
+          cbn in H9.
+          inv H9.
+        }
+
+        destruct H6 as [[] | H6].
+        specialize (H6 _ eq_refl).
+        cbn in H6.
+        rewrite <- H6 in H3.
+        cbn in H3.
+        destruct H3 as [[] | H3].
+        specialize (H3 _ eq_refl).
+
+        specialize (IHHeqo (success_unERR_UB_OOM (DVALUE_Vector x5))).
+        forward IHHeqo.
+        { cbn.
+          red.
+          exists (success_unERR_UB_OOM x5).
+          exists (fun xs => ret (DVALUE_Vector xs)).
+          split; cbn; eauto.
+        }
+
+        repeat red in IHHeqo.
+        destruct IHHeqo as (?&?&?&?&?).
+        destruct_err_ub_oom x2; cbn in H8; inv H8.
+        destruct H9 as [[] | H9].
+        specialize (H9 _ eq_refl).
+        cbn in H9.
+        rewrite <- H9 in H11.
+        inv H11.
+        rewrite <- H6 in H5.
+        inv H5.
+
+        repeat red.
+        exists (ret (fmap fin_to_inf_dvalue (x0::x5))).
+        exists (fun xs => ret (IS1.LP.Events.DV.DVALUE_Vector xs)).
+        rewrite map_monad_unfold.
+        split; cbn; eauto.
+        2: {
+          rewrite <- H11; cbn.
+          rewrite <- H3; cbn.
+          split; cbn; eauto.
+          rewrite fin_to_inf_dvalue_vector.
+          cbn.
+          reflexivity.
+        }
+
+        exists (fmap fin_to_inf_dvalue (success_unERR_UB_OOM x0)).
+        exists (fun _ => ret (fmap fin_to_inf_dvalue (x0 :: x5))).
+        split; cbn; eauto.
+        split; cbn; eauto.
+        right.
+        intros; subst.
+        red.
+
+        exists (success_unERR_UB_OOM x7).
+        exists (fun _ => ret (fmap fin_to_inf_dvalue (x0 :: x5))).
+        split; cbn; eauto.
+        split; cbn; eauto.
+        right.
+        intros; subst.
+        rewrite fin_to_inf_dvalue_vector in H10.
+        inv H10.
+        { (* TODO: should probably make this a lemma... *)
+          induction x5; eauto.
+        }
+    - (* IBinop *)
+      red; intros dv_fin CONC_FIN.
+      red in REF.
+      cbn in REF.
+      break_match_hyp_inv.
+      break_match_hyp_inv.
+
+      unfold uvalue_concretize_u_fin_inf_inclusion in IHuv_inf1, IHuv_inf2.
+
+      specialize (IHuv_inf1 u Heqo).
+      specialize (IHuv_inf2 u0 Heqo0).
+
+      red.
+      rewrite IS1.LLVM.MEM.CP.CONCBASE.concretize_uvalueM_equation.
+
+      red in CONC_FIN.
+      rewrite IS2.LLVM.MEM.CP.CONCBASE.concretize_uvalueM_equation in CONC_FIN.
+
+      repeat red in CONC_FIN.
+      destruct CONC_FIN as (?&?&?&?&?).
+
+      specialize (IHuv_inf1 _ H).
+      destruct_err_ub_oom x; cbn in H0; inv H0.
+
+      { (* OOM *)
+        exists (OOM_unERR_UB_OOM oom_x).
+        eexists.
+        split; cbn; eauto.
+      }
+
+      { (* UB *)
+        exists (UB_unERR_UB_OOM ub_x).
+        eexists.
+        split; cbn; eauto.
+      }
+
+      { (* Err *)
+        exists (ERR_unERR_UB_OOM err_x).
+        eexists.
+        split; cbn; eauto.
+      }
+
+      destruct H1 as [[] | H1].
+      specialize (H1 _ eq_refl).
+      cbn in H1.
+      repeat red in H1.
+      destruct H1 as (?&?&?&?&?).
+
+      specialize (IHuv_inf2 _ H0).
+
+      repeat red.
+      exists (fmap fin_to_inf_dvalue (success_unERR_UB_OOM x1)).
+      exists (fun _ => fmap fin_to_inf_dvalue (x0 x1)).
+      split; cbn; eauto.
+      split; cbn; eauto.
+      right.
+      intros; subst.
+      red.
+
+      exists (fmap fin_to_inf_dvalue x).
+      eexists.
+
+      destruct_err_ub_oom x; cbn in H1; rewrite <- H1 in H2; inv H2;
+        rewrite <- H1;
+        cbn;
+        split; cbn; eauto.
+
+      destruct H3 as [[] | H3].
+      specialize (H3 _ eq_refl).
+      rewrite <- H3 in H1.
+
+      remember (eval_iop iop x1 x3) as x1x3.
+      destruct_err_ub_oom x1x3; inv H1;
+      rewrite <- H3; cbn.
+  (*     cbn in H1. *)
+
+  (*     apply IHuv_inf1 in H. *)
+  (*     apply IHuv_inf2 in H0. *)
+
+  (*     repeat red. *)
+  (*     exists (ret (fin_to_inf_dvalue x1)). *)
+  (*     exists (fun dv_inf => (fmap fin_to_inf_dvalue (x0 x1))). *)
+  (*     cbn. *)
+  (*     rewrite <- H1. *)
+  (*     cbn. *)
+  (*     split; eauto. *)
+  (*     split; eauto. *)
+
+  (*     right. *)
+  (*     intros a H3. *)
+  (*     repeat red. *)
+  (*     exists (ret (fin_to_inf_dvalue x3)). *)
+  (*     exists (fun dv_inf => (fmap fin_to_inf_dvalue (x2 x3))). *)
+  (*     cbn. *)
+  (*     rewrite <- H2. *)
+  (*     cbn. *)
+  (*     split; eauto. *)
+  (*     split; eauto. *)
+
+  (*     right. *)
+  (*     intros a0 H4. *)
+
+  (*     eapply eval_iop_fin_inf; eauto. *)
+  (*   - (* ICmp *) *)
+  (*     red; intros dv_fin CONC_FIN. *)
+  (*     red in REF. *)
+  (*     cbn in REF. *)
+  (*     break_match_hyp_inv. *)
+  (*     break_match_hyp_inv. *)
+
+  (*     unfold uvalue_concretize_fin_inf_inclusion in IHuv_inf1, IHuv_inf2. *)
+
+  (*     specialize (IHuv_inf1 u Heqo). *)
+  (*     specialize (IHuv_inf2 u0 Heqo0). *)
+
+  (*     rewrite IS1.MEM.CP.CONC.concretize_equation. *)
+  (*     red. *)
+  (*     rewrite IS1.LLVM.MEM.CP.CONCBASE.concretize_uvalueM_equation. *)
+
+  (*     rewrite IS2.MEM.CP.CONC.concretize_equation in CONC_FIN. *)
+  (*     red in CONC_FIN. *)
+  (*     rewrite IS2.LLVM.MEM.CP.CONCBASE.concretize_uvalueM_equation in CONC_FIN. *)
+
+  (*     repeat red in CONC_FIN. *)
+  (*     destruct CONC_FIN as (?&?&?&?&?). *)
+  (*     destruct_err_ub_oom x; cbn in H0; inv H0. *)
+  (*     destruct H1 as [[] | H1]. *)
+  (*     specialize (H1 _ eq_refl). *)
+  (*     cbn in H1. *)
+  (*     repeat red in H1. *)
+  (*     destruct H1 as (?&?&?&?&?). *)
+  (*     destruct_err_ub_oom x; cbn in H1; rewrite <- H1 in H3; inv H3. *)
+  (*     destruct H2 as [[] | H2]. *)
+  (*     specialize (H2 _ eq_refl). *)
+  (*     rewrite <- H2 in H5, H1. *)
+
+  (*     remember (eval_icmp cmp0 x1 x3) as x1x3. *)
+  (*     destruct_err_ub_oom x1x3; inv H5. *)
+  (*     cbn in H1. *)
+
+  (*     apply IHuv_inf1 in H. *)
+  (*     apply IHuv_inf2 in H0. *)
+
+  (*     repeat red. *)
+  (*     exists (ret (fin_to_inf_dvalue x1)). *)
+  (*     exists (fun dv_inf => (fmap fin_to_inf_dvalue (x0 x1))). *)
+  (*     cbn. *)
+  (*     rewrite <- H1. *)
+  (*     cbn. *)
+  (*     split; eauto. *)
+  (*     split; eauto. *)
+
+  (*     right. *)
+  (*     intros a H3. *)
+  (*     repeat red. *)
+  (*     exists (ret (fin_to_inf_dvalue x3)). *)
+  (*     exists (fun dv_inf => (fmap fin_to_inf_dvalue (x2 x3))). *)
+  (*     cbn. *)
+  (*     rewrite <- H2. *)
+  (*     cbn. *)
+  (*     split; eauto. *)
+  (*     split; eauto. *)
+
+  (*     right. *)
+  (*     intros a0 H4. *)
+
+  (*     eapply eval_icmp_fin_inf; eauto. *)
+  (*   - (* FBinop *) *)
+  (*     red; intros dv_fin CONC_FIN. *)
+  (*     red in REF. *)
+  (*     cbn in REF. *)
+  (*     break_match_hyp_inv. *)
+  (*     break_match_hyp_inv. *)
+
+  (*     unfold uvalue_concretize_fin_inf_inclusion in IHuv_inf1, IHuv_inf2. *)
+
+  (*     specialize (IHuv_inf1 u Heqo). *)
+  (*     specialize (IHuv_inf2 u0 Heqo0). *)
+
+  (*     rewrite IS1.MEM.CP.CONC.concretize_equation. *)
+  (*     red. *)
+  (*     rewrite IS1.LLVM.MEM.CP.CONCBASE.concretize_uvalueM_equation. *)
+
+  (*     rewrite IS2.MEM.CP.CONC.concretize_equation in CONC_FIN. *)
+  (*     red in CONC_FIN. *)
+  (*     rewrite IS2.LLVM.MEM.CP.CONCBASE.concretize_uvalueM_equation in CONC_FIN. *)
+
+  (*     repeat red in CONC_FIN. *)
+  (*     destruct CONC_FIN as (?&?&?&?&?). *)
+  (*     destruct_err_ub_oom x; cbn in H0; inv H0. *)
+  (*     destruct H1 as [[] | H1]. *)
+  (*     specialize (H1 _ eq_refl). *)
+  (*     cbn in H1. *)
+  (*     repeat red in H1. *)
+  (*     destruct H1 as (?&?&?&?&?). *)
+  (*     destruct_err_ub_oom x; cbn in H1; rewrite <- H1 in H3; inv H3. *)
+  (*     destruct H2 as [[] | H2]. *)
+  (*     specialize (H2 _ eq_refl). *)
+  (*     rewrite <- H2 in H5, H1. *)
+
+  (*     remember (eval_fop fop x1 x3) as x1x3. *)
+  (*     destruct_err_ub_oom x1x3; inv H5. *)
+  (*     cbn in H1. *)
+
+  (*     apply IHuv_inf1 in H. *)
+  (*     apply IHuv_inf2 in H0. *)
+
+  (*     repeat red. *)
+  (*     exists (ret (fin_to_inf_dvalue x1)). *)
+  (*     exists (fun dv_inf => (fmap fin_to_inf_dvalue (x0 x1))). *)
+  (*     cbn. *)
+  (*     rewrite <- H1. *)
+  (*     cbn. *)
+  (*     split; eauto. *)
+  (*     split; eauto. *)
+
+  (*     right. *)
+  (*     intros a H3. *)
+  (*     repeat red. *)
+  (*     exists (ret (fin_to_inf_dvalue x3)). *)
+  (*     exists (fun dv_inf => (fmap fin_to_inf_dvalue (x2 x3))). *)
+  (*     cbn. *)
+  (*     rewrite <- H2. *)
+  (*     cbn. *)
+  (*     split; eauto. *)
+  (*     split; eauto. *)
+
+  (*     right. *)
+  (*     intros a0 H4. *)
+
+  (*     eapply eval_fop_fin_inf; eauto. *)
+  (*   - (* fcmp *) *)
+  (*     red; intros dv_fin CONC_FIN. *)
+  (*     red in REF. *)
+  (*     cbn in REF. *)
+  (*     break_match_hyp_inv. *)
+  (*     break_match_hyp_inv. *)
+
+  (*     unfold uvalue_concretize_fin_inf_inclusion in IHuv_inf1, IHuv_inf2. *)
+
+  (*     specialize (IHuv_inf1 u Heqo). *)
+  (*     specialize (IHuv_inf2 u0 Heqo0). *)
+
+  (*     rewrite IS1.MEM.CP.CONC.concretize_equation. *)
+  (*     red. *)
+  (*     rewrite IS1.LLVM.MEM.CP.CONCBASE.concretize_uvalueM_equation. *)
+
+  (*     rewrite IS2.MEM.CP.CONC.concretize_equation in CONC_FIN. *)
+  (*     red in CONC_FIN. *)
+  (*     rewrite IS2.LLVM.MEM.CP.CONCBASE.concretize_uvalueM_equation in CONC_FIN. *)
+
+  (*     repeat red in CONC_FIN. *)
+  (*     destruct CONC_FIN as (?&?&?&?&?). *)
+  (*     destruct_err_ub_oom x; cbn in H0; inv H0. *)
+  (*     destruct H1 as [[] | H1]. *)
+  (*     specialize (H1 _ eq_refl). *)
+  (*     cbn in H1. *)
+  (*     repeat red in H1. *)
+  (*     destruct H1 as (?&?&?&?&?). *)
+  (*     destruct_err_ub_oom x; cbn in H1; rewrite <- H1 in H3; inv H3. *)
+  (*     destruct H2 as [[] | H2]. *)
+  (*     specialize (H2 _ eq_refl). *)
+  (*     rewrite <- H2 in H5, H1. *)
+
+  (*     remember (eval_fcmp cmp0 x1 x3) as x1x3. *)
+  (*     destruct_err_ub_oom x1x3; inv H5. *)
+  (*     cbn in H1. *)
+
+  (*     apply IHuv_inf1 in H. *)
+  (*     apply IHuv_inf2 in H0. *)
+
+  (*     repeat red. *)
+  (*     exists (ret (fin_to_inf_dvalue x1)). *)
+  (*     exists (fun dv_inf => (fmap fin_to_inf_dvalue (x0 x1))). *)
+  (*     cbn. *)
+  (*     rewrite <- H1. *)
+  (*     cbn. *)
+  (*     split; eauto. *)
+  (*     split; eauto. *)
+
+  (*     right. *)
+  (*     intros a H3. *)
+  (*     repeat red. *)
+  (*     exists (ret (fin_to_inf_dvalue x3)). *)
+  (*     exists (fun dv_inf => (fmap fin_to_inf_dvalue (x2 x3))). *)
+  (*     cbn. *)
+  (*     rewrite <- H2. *)
+  (*     cbn. *)
+  (*     split; eauto. *)
+  (*     split; eauto. *)
+
+  (*     right. *)
+  (*     intros a0 H4. *)
+
+  (*     eapply eval_fcmp_fin_inf; eauto. *)
+  (*   - (* Conversion *) *)
+  (*     red; intros dv_fin CONC_FIN. *)
+  (*     red in REF. *)
+  (*     cbn in REF. *)
+  (*     break_match_hyp_inv. *)
+
+  (*     specialize (IHuv_inf _ Heqo). *)
+  (*     unfold uvalue_concretize_fin_inf_inclusion in IHuv_inf. *)
+
+  (*     rewrite IS1.MEM.CP.CONC.concretize_equation. *)
+  (*     red. *)
+  (*     rewrite IS1.LLVM.MEM.CP.CONCBASE.concretize_uvalueM_equation. *)
+
+  (*     rewrite IS2.MEM.CP.CONC.concretize_equation in CONC_FIN. *)
+  (*     red in CONC_FIN. *)
+  (*     rewrite IS2.LLVM.MEM.CP.CONCBASE.concretize_uvalueM_equation in CONC_FIN. *)
+
+  (*     repeat red in CONC_FIN. *)
+  (*     destruct CONC_FIN as (?&?&?&?&?). *)
+  (*     destruct_err_ub_oom x; cbn in H0; inv H0. *)
+  (*     destruct H1 as [[] | H1]. *)
+  (*     specialize (H1 _ eq_refl). *)
+  (*     cbn in H1. *)
+
+  (*     specialize (IHuv_inf _ H). *)
+  (*     repeat red. *)
+  (*     exists (ret (fin_to_inf_dvalue x1)). *)
+  (*     exists (fun _ => (fmap fin_to_inf_dvalue (x0 x1))). *)
+  (*     cbn; rewrite H3; cbn. *)
+  (*     split; eauto. *)
+  (*     split; eauto. *)
+
+  (*     right; intros ? ?; subst. *)
+  (*     break_match_hyp. *)
+  (*     { (* Conv_Pure *) *)
+  (*       pose proof get_conv_case_pure_fin_inf _ _ _ _ _ Heqc as CONV. *)
+  (*       rewrite CONV. *)
+  (*       rewrite <- H1 in H3; inv H3; auto. *)
+  (*     } *)
+
+  (*     { (* Conv_ItoP *) *)
+  (*       break_match_hyp; *)
+  (*         rewrite <- H1 in H3; inv H3. *)
+
+  (*       pose proof get_conv_case_itop_fin_inf _ _ _ _ _ Heqc as CONV. *)
+  (*       rewrite CONV. *)
+  (*       admit. *)
+  (*     } *)
+
+  (*     { (* Conv_PtoI *) *)
+  (*       admit. *)
+  (*     } *)
+
+  (*     { (* Conv_Illegal *) *)
+  (*       exfalso. *)
+  (*       rewrite <- H1 in H3; inv H3. *)
+  (*     } *)
+  (*   - (* GetElementPtr *) *)
+  (*     red; intros dv_fin CONC_FIN. *)
+  (*     red in REF. *)
+  (*     cbn in REF. *)
+  (*     break_match_hyp_inv. *)
+  (*     break_match_hyp_inv. *)
+
+  (*     pose proof (IHuv_inf u Heqo) as IHuv_inf_u. *)
+  (*     unfold uvalue_concretize_fin_inf_inclusion in IHuv_inf_u. *)
+
+  (*     rewrite IS2.MEM.CP.CONC.concretize_equation in CONC_FIN. *)
+  (*     red in CONC_FIN. *)
+  (*     rewrite IS2.LLVM.MEM.CP.CONCBASE.concretize_uvalueM_equation in CONC_FIN. *)
+
+  (*     repeat red in CONC_FIN. *)
+  (*     destruct CONC_FIN as (?&?&?&?&?). *)
+  (*     destruct_err_ub_oom x; cbn in H1; inv H1. *)
+  (*     destruct H2 as [[] | H2]. *)
+  (*     specialize (H2 _ eq_refl). *)
+  (*     cbn in H2. *)
+  (*     repeat red in H2. *)
+  (*     destruct H2 as (?&?&?&?&?). *)
+  (*     destruct_err_ub_oom x; cbn in H2; rewrite <- H2 in H4; inv H4. *)
+  (*     destruct H3 as [[] | H3]. *)
+  (*     specialize (H3 _ eq_refl). *)
+  (*     break_match_hyp; try rewrite <- H3 in H6; inv H6. *)
+  (*     break_match_hyp; try rewrite <- H3 in H5; inv H5. *)
+  (*     rewrite <- H3 in H2; cbn in H2. *)
+
+  (*     specialize (IHuv_inf_u _ H0). *)
+  (*     destruct x1; cbn in Heqs; inv Heqs. *)
+  (*     break_match_hyp_inv. *)
+  (*     break_match_hyp_inv. *)
+
+  (*     pose proof addr_convert_succeeds a as (a'&AA'). *)
+  (*     pose proof addr_convert_succeeds a0 as (a0'&A0A0'). *)
+  (*     epose proof (handle_gep_addr_fin_inf _ _ _ _ _ _ _ Heqs AA' A0A0' eq_refl). *)
+
+  (*     rewrite IS1.MEM.CP.CONC.concretize_equation. *)
+  (*     red. *)
+  (*     rewrite IS1.LLVM.MEM.CP.CONCBASE.concretize_uvalueM_equation. *)
+
+  (*     repeat red. *)
+  (*     exists (ret (fin_to_inf_dvalue (DVALUE_Addr a))). *)
+  (*     exists (fun dv_inf => (fmap fin_to_inf_dvalue (x0 (DVALUE_Addr a)))). *)
+  (*     rewrite <- H2. *)
+  (*     split; eauto. *)
+  (*     split; cbn; eauto. *)
+
+  (*     right. *)
+  (*     intros a1 ?; subst. *)
+  (*     repeat red. *)
+  (*     exists (ret (fmap fin_to_inf_dvalue x3)). *)
+  (*     exists (fun dv_inf => (fmap fin_to_inf_dvalue (x2 x3))). *)
+  (*     cbn. *)
+  (*     split; eauto. *)
+  (*     { clear - H H1 Heqo0. *)
+  (*       apply map_monad_oom_Forall2 in Heqo0. *)
+  (*       generalize dependent x3. *)
+  (*       induction Heqo0; intros x3 H1. *)
+  (*       - cbn in *; inv H1; cbn; auto. *)
+  (*       - forward IHHeqo0. *)
+  (*         { intros idx H2 uv_fin H3. *)
+  (*           eapply H; eauto; right; auto. *)
+  (*         } *)
+
+  (*         rewrite map_monad_unfold in H1. *)
+  (*         repeat red in H1. *)
+  (*         destruct H1 as (?&?&?&?&?). *)
+  (*         destruct_err_ub_oom x0; inv H2. *)
+  (*         destruct H3 as [[] | H3]. *)
+  (*         specialize (H3 _ eq_refl). *)
+
+  (*         repeat red in H3. *)
+  (*         destruct H3 as (?&?&?&?&?). *)
+  (*         rewrite <- H3 in H5. *)
+  (*         destruct_err_ub_oom x0; inv H5. *)
+
+  (*         destruct H4 as [[] | H4]. *)
+  (*         specialize (H4 _ eq_refl). *)
+  (*         cbn in H4. *)
+
+  (*         rewrite <- H4 in H7; inv H7. *)
+  (*         cbn in H3; rewrite <- H4 in H3; inv H3. *)
+
+  (*         specialize (IHHeqo0 _ H2). *)
+  (*         rewrite map_monad_unfold. *)
+  (*         repeat red. *)
+
+  (*         pose proof (H x (or_introl eq_refl) _ H0 _ H1). *)
+
+  (*         exists (ret (fin_to_inf_dvalue x2)). *)
+  (*         exists (fun dv_inf => fmap (fmap fin_to_inf_dvalue) (x1 x2)). *)
+
+  (*         cbn; rewrite <- H6; cbn. *)
+  (*         split; eauto. *)
+  (*         split; eauto. *)
+
+  (*         right. *)
+  (*         intros a ?; subst. *)
+  (*         repeat red. *)
+  (*         exists (ret (fmap fin_to_inf_dvalue x5)). *)
+  (*         exists (fun dv_inf => (fmap (fmap fin_to_inf_dvalue) (x4 x5))). *)
+
+  (*         cbn; rewrite <- H4; cbn. *)
+  (*         split; eauto. *)
+  (*         split; eauto. *)
+
+  (*         right. *)
+  (*         intros a ?; subst. *)
+  (*         auto. *)
+  (*     } *)
+
+  (*     cbn; rewrite <- H3; cbn. *)
+  (*     split; eauto. *)
+
+  (*     right. *)
+  (*     intros a1 ?; subst. *)
+  (*     unfold fin_to_inf_dvalue at 1. *)
+  (*     break_inner_match_goal; clear Heqs0; destruct p; clear e0. *)
+  (*     cbn in e. *)
+  (*     rewrite AA' in e. *)
+  (*     inv e. *)
+  (*     cbn. *)
+
+  (*     replace (map fin_to_inf_dvalue x3) with (fmap fin_to_inf_dvalue x3) in H4 by reflexivity. *)
+  (*     cbn in H4. *)
+  (*     rewrite H4. *)
+
+  (*     unfold fin_to_inf_dvalue. *)
+  (*     break_match_goal; clear Heqs0; destruct p; clear e0. *)
+  (*     cbn in e. *)
+  (*     rewrite A0A0' in e. *)
+  (*     inv e. *)
+  (*     reflexivity. *)
+  (*   - (* ExtractElement *) *)
+  (*     red; intros dv_fin CONC_FIN. *)
+  (*     red in REF. *)
+  (*     cbn in REF. *)
+  (*     break_match_hyp_inv. *)
+  (*     break_match_hyp_inv. *)
+
+  (*     pose proof (IHuv_inf1 u Heqo) as IHuv_inf_u. *)
+  (*     pose proof (IHuv_inf2 u0 Heqo0) as IHuv_inf_u0. *)
+
+  (*     unfold uvalue_concretize_fin_inf_inclusion in IHuv_inf_u, IHuv_inf_u0. *)
+
+  (*     rewrite IS2.MEM.CP.CONC.concretize_equation in CONC_FIN. *)
+  (*     red in CONC_FIN. *)
+  (*     rewrite IS2.LLVM.MEM.CP.CONCBASE.concretize_uvalueM_equation in CONC_FIN. *)
+
+  (*     repeat red in CONC_FIN. *)
+  (*     destruct CONC_FIN as (?&?&?&?&?). *)
+  (*     destruct_err_ub_oom x; inv H0. *)
+  (*     destruct H1 as [[] | H1]. *)
+  (*     specialize (H1 _ eq_refl). *)
+  (*     cbn in H1. *)
+  (*     repeat red in H1. *)
+  (*     destruct H1 as (?&?&?&?&?). *)
+  (*     destruct_err_ub_oom x; cbn in H1; rewrite <- H1 in H3; inv H3. *)
+  (*     destruct H2 as [[] | H2]. *)
+  (*     specialize (H2 _ eq_refl). *)
+
+  (*     repeat red in H2. *)
+  (*     destruct H2 as (?&?&?&?&?). *)
+  (*     destruct_err_ub_oom x; cbn in H3; rewrite <- H3 in H5; inv H5. *)
+  (*     destruct H4 as [[] | H4]. *)
+  (*     specialize (H4 _ eq_refl). *)
+
+  (*     remember (x4 x5) as x4x5. *)
+  (*     destruct_err_ub_oom x4x5; inv H7. *)
+  (*     cbn in H3. *)
+  (*     rewrite <- H3 in H1. *)
+  (*     cbn in H1. *)
+
+  (*     break_match_hyp_inv. *)
+
+  (*     specialize (IHuv_inf_u _ H). *)
+  (*     specialize (IHuv_inf_u0 _ H0). *)
+
+  (*     rewrite IS1.MEM.CP.CONC.concretize_equation. *)
+  (*     red. *)
+  (*     rewrite IS1.LLVM.MEM.CP.CONCBASE.concretize_uvalueM_equation. *)
+
+  (*     repeat red. *)
+  (*     exists (ret (fin_to_inf_dvalue x1)). *)
+  (*     exists (fun dv_inf => (fmap fin_to_inf_dvalue (x0 x1))). *)
+  (*     cbn. *)
+  (*     rewrite <- H1. *)
+  (*     cbn. *)
+  (*     split; eauto. *)
+  (*     split; eauto. *)
+
+  (*     right. *)
+  (*     intros a ?; subst. *)
+  (*     repeat red. *)
+  (*     exists (ret (fin_to_inf_dvalue x3)). *)
+  (*     exists (fun dv_inf => (fmap fin_to_inf_dvalue (x2 x3))). *)
+  (*     cbn; rewrite <- H3; cbn. *)
+  (*     split; eauto. *)
+  (*     split; eauto. *)
+
+  (*     right. *)
+  (*     intros a ?; subst. *)
+  (*     repeat red. *)
+  (*     exists (ret x5). *)
+  (*     exists (fun x5 => fmap fin_to_inf_dvalue (x4 x5)). *)
+  (*     cbn; rewrite <- Heqx4x5; cbn. *)
+  (*     split; eauto. *)
+  (*     split; eauto. *)
+
+  (*     right. *)
+  (*     intros a ?; subst. *)
+  (*     cbn; rewrite <- Heqx4x5; cbn. *)
+
+  (*     eapply index_into_vec_dv_fin_inf; eauto. *)
+  (*   - (* InsertElement *) *)
+  (*     red; intros dv_fin CONC_FIN. *)
+  (*     red in REF. *)
+  (*     cbn in REF. *)
+  (*     break_match_hyp_inv. *)
+  (*     break_match_hyp_inv. *)
+  (*     break_match_hyp_inv. *)
+
+  (*     pose proof (IHuv_inf1 u Heqo) as IHuv_inf_u. *)
+  (*     pose proof (IHuv_inf2 u0 Heqo0) as IHuv_inf_u0. *)
+  (*     pose proof (IHuv_inf3 u1 Heqo1) as IHuv_inf_u1. *)
+
+  (*     unfold uvalue_concretize_fin_inf_inclusion in IHuv_inf_u, IHuv_inf_u0, IHuv_inf_u1. *)
+
+  (*     rewrite IS2.MEM.CP.CONC.concretize_equation in CONC_FIN. *)
+  (*     red in CONC_FIN. *)
+  (*     rewrite IS2.LLVM.MEM.CP.CONCBASE.concretize_uvalueM_equation in CONC_FIN. *)
+
+  (*     repeat red in CONC_FIN. *)
+  (*     destruct CONC_FIN as (?&?&?&?&?). *)
+  (*     destruct_err_ub_oom x; inv H0. *)
+  (*     destruct H1 as [[] | H1]. *)
+  (*     specialize (H1 _ eq_refl). *)
+  (*     cbn in H1. *)
+
+  (*     repeat red in H1. *)
+  (*     destruct H1 as (?&?&?&?&?). *)
+  (*     destruct_err_ub_oom x; cbn in H1; rewrite <- H1 in H3; inv H3. *)
+  (*     destruct H2 as [[] | H2]. *)
+  (*     specialize (H2 _ eq_refl). *)
+
+  (*     repeat red in H2. *)
+  (*     destruct H2 as (?&?&?&?&?). *)
+  (*     destruct_err_ub_oom x; cbn in H3; rewrite <- H3 in H5; inv H5. *)
+  (*     destruct H4 as [[] | H4]. *)
+  (*     specialize (H4 _ eq_refl). *)
+
+  (*     remember (x4 x5) as x4x5. *)
+  (*     destruct_err_ub_oom x4x5; inv H7. *)
+  (*     cbn in H3. *)
+  (*     rewrite <- H3 in H1. *)
+  (*     cbn in H1. *)
+
+  (*     specialize (IHuv_inf_u _ H). *)
+  (*     specialize (IHuv_inf_u0 _ H2). *)
+  (*     specialize (IHuv_inf_u1 _ H0). *)
+
+  (*     rewrite IS1.MEM.CP.CONC.concretize_equation. *)
+  (*     red. *)
+  (*     rewrite IS1.LLVM.MEM.CP.CONCBASE.concretize_uvalueM_equation. *)
+
+  (*     repeat red. *)
+  (*     exists (ret (fin_to_inf_dvalue x1)). *)
+  (*     exists (fun dv_inf => (fmap fin_to_inf_dvalue (x0 x1))). *)
+  (*     cbn. *)
+  (*     rewrite <- H1. *)
+  (*     cbn. *)
+  (*     split; eauto. *)
+  (*     split; eauto. *)
+
+  (*     right. *)
+  (*     intros a ?; subst. *)
+  (*     repeat red. *)
+  (*     exists (ret (fin_to_inf_dvalue x3)). *)
+  (*     exists (fun dv_inf => (fmap fin_to_inf_dvalue (x2 x3))). *)
+  (*     cbn; rewrite <- H3; cbn. *)
+  (*     split; eauto. *)
+  (*     split; eauto. *)
+
+  (*     right. *)
+  (*     intros a ?; subst. *)
+  (*     repeat red. *)
+  (*     exists (ret (fin_to_inf_dvalue x5)). *)
+  (*     exists (fun dv_inf => (fmap fin_to_inf_dvalue (x4 x5))). *)
+  (*     cbn; rewrite <- Heqx4x5; cbn. *)
+  (*     split; eauto. *)
+  (*     split; eauto. *)
+
+  (*     right. *)
+  (*     intros a ?; subst. *)
+
+  (*     eapply insert_into_vec_dv_fin_inf; eauto. *)
+  (*   - (* ShuffleVector *) *)
+  (*     red; intros dv_fin CONC_FIN. *)
+  (*     red in REF. *)
+  (*     cbn in REF. *)
+  (*     break_match_hyp_inv. *)
+  (*     break_match_hyp_inv. *)
+  (*     break_match_hyp_inv. *)
+
+  (*     pose proof (IHuv_inf1 u Heqo) as IHuv_inf_u. *)
+  (*     pose proof (IHuv_inf2 u0 Heqo0) as IHuv_inf_u0. *)
+  (*     pose proof (IHuv_inf3 u1 Heqo1) as IHuv_inf_u1. *)
+
+  (*     unfold uvalue_concretize_fin_inf_inclusion in IHuv_inf_u, IHuv_inf_u0, IHuv_inf_u1. *)
+
+  (*     rewrite IS2.MEM.CP.CONC.concretize_equation in CONC_FIN. *)
+  (*     red in CONC_FIN. *)
+  (*     rewrite IS2.LLVM.MEM.CP.CONCBASE.concretize_uvalueM_equation in CONC_FIN. *)
+  (*     inv CONC_FIN. *)
+  (*   - (* ExtractValue *) *)
+  (*     red; intros dv_fin CONC_FIN. *)
+  (*     red in REF. *)
+  (*     cbn in REF. *)
+  (*     break_match_hyp_inv. *)
+
+  (*     rewrite IS2.MEM.CP.CONC.concretize_equation in CONC_FIN. *)
+  (*     red in CONC_FIN. *)
+  (*     rewrite IS2.LLVM.MEM.CP.CONCBASE.concretize_uvalueM_equation in CONC_FIN. *)
+  (*     cbn in CONC_FIN. *)
+  (*     repeat red in CONC_FIN. *)
+
+  (*     destruct CONC_FIN as (?&?&?&?&?). *)
+  (*     destruct_err_ub_oom x; inv H0. *)
+  (*     destruct H1 as [[] | H1]. *)
+  (*     specialize (H1 _ eq_refl). *)
+
+  (*     remember (x0 x1) as x0x1. *)
+  (*     destruct_err_ub_oom x0x1; inv H3. *)
+  (*     apply extract_value_loop_fin_inf_succeeds in H1. *)
+
+  (*     rewrite IS1.MEM.CP.CONC.concretize_equation; *)
+  (*       red; rewrite IS1.LLVM.MEM.CP.CONCBASE.concretize_uvalueM_equation; *)
+  (*       cbn; repeat red. *)
+
+  (*     exists (ret (fin_to_inf_dvalue x1)). *)
+  (*     exists (fun dv_inf => (fmap fin_to_inf_dvalue (x0 x1))). *)
+  (*     cbn; rewrite <- Heqx0x1; cbn. *)
+  (*     split. *)
+  (*     eapply IHuv_inf; eauto. *)
+  (*     split; eauto. *)
+
+  (*     right. *)
+  (*     intros a ?; subst. *)
+  (*     auto. *)
+  (*   - (* InsertValue *) *)
+  (*     red; intros dv_fin CONC_FIN. *)
+  (*     red in REF. *)
+  (*     cbn in REF. *)
+  (*     break_match_hyp_inv. *)
+  (*     break_match_hyp_inv. *)
+
+  (*     pose proof (IHuv_inf1 u Heqo) as IHuv_inf_u. *)
+  (*     pose proof (IHuv_inf2 u0 Heqo0) as IHuv_inf_u0. *)
+  (*     red in IHuv_inf_u, IHuv_inf_u0. *)
+
+  (*     rewrite IS2.MEM.CP.CONC.concretize_equation in CONC_FIN. *)
+  (*     red in CONC_FIN. *)
+  (*     rewrite IS2.LLVM.MEM.CP.CONCBASE.concretize_uvalueM_equation in CONC_FIN. *)
+  (*     cbn in CONC_FIN. *)
+
+  (*     repeat red in CONC_FIN. *)
+  (*     destruct CONC_FIN as (?&?&?&?&?). *)
+  (*     destruct_err_ub_oom x; inv H0. *)
+  (*     destruct H1 as [[] | H1]. *)
+  (*     specialize (H1 _ eq_refl). *)
+
+  (*     repeat red in H1. *)
+  (*     destruct H1 as (?&?&?&?&?). *)
+  (*     rewrite <- H1 in H3. *)
+  (*     destruct_err_ub_oom x; inv H3. *)
+  (*     cbn in H1. *)
+  (*     destruct H2 as [[] | H2]. *)
+  (*     specialize (H2 _ eq_refl). *)
+
+  (*     specialize (IHuv_inf_u _ H). *)
+  (*     specialize (IHuv_inf_u0 _ H0). *)
+
+  (*     rewrite IS1.MEM.CP.CONC.concretize_equation; *)
+  (*       red; rewrite IS1.LLVM.MEM.CP.CONCBASE.concretize_uvalueM_equation; *)
+  (*       cbn; repeat red. *)
+
+  (*     exists (ret (fin_to_inf_dvalue x1)). *)
+  (*     exists (fun dv_inf => (fmap fin_to_inf_dvalue (x0 x1))). *)
+  (*     cbn; rewrite <- H1, H5; cbn. *)
+  (*     split; eauto. *)
+  (*     split; eauto. *)
+
+  (*     right. *)
+  (*     intros a ?; subst. *)
+  (*     repeat red. *)
+
+  (*     exists (ret (fin_to_inf_dvalue x3)). *)
+  (*     exists (fun dv_inf => (fmap fin_to_inf_dvalue (x2 x3))). *)
+  (*     cbn; rewrite H5; cbn. *)
+  (*     split; eauto. *)
+  (*     split; eauto. *)
+
+  (*     right. *)
+  (*     intros a ?; subst. *)
+  (*     eapply insert_value_loop_fin_inf_succeeds in H2. *)
+  (*     setoid_rewrite H2. *)
+  (*     remember (x2 x3) as x2x3. *)
+  (*     destruct_err_ub_oom x2x3; inv H5. *)
+  (*     reflexivity. *)
+  (*   - (* Select *) *)
+  (*     red; intros dv_fin CONC_FIN. *)
+  (*     red in REF. *)
+  (*     cbn in REF. *)
+  (*     break_match_hyp_inv. *)
+  (*     break_match_hyp_inv. *)
+  (*     break_match_hyp_inv. *)
+
+  (*     pose proof (IHuv_inf1 u Heqo) as IHuv_inf_u. *)
+  (*     pose proof (IHuv_inf2 u0 Heqo0) as IHuv_inf_u0. *)
+  (*     pose proof (IHuv_inf3 u1 Heqo1) as IHuv_inf_u1. *)
+  (*     red in IHuv_inf_u, IHuv_inf_u0, IHuv_inf_u1. *)
+
+  (*     rewrite IS2.MEM.CP.CONC.concretize_equation in CONC_FIN. *)
+  (*     red in CONC_FIN. *)
+  (*     rewrite IS2.LLVM.MEM.CP.CONCBASE.concretize_uvalueM_equation in CONC_FIN. *)
+  (*     cbn in CONC_FIN. *)
+
+  (*     repeat red in CONC_FIN. *)
+  (*     destruct CONC_FIN as (?&?&?&?&?). *)
+  (*     destruct_err_ub_oom x; inv H0. *)
+  (*     destruct H1 as [[] | H1]. *)
+  (*     specialize (H1 _ eq_refl). *)
+
+  (*     remember (x0 x1) as x0x1. *)
+  (*     destruct_err_ub_oom x0x1; inv H3. *)
+  (*     pose proof eval_select_fin_inf x1 u0 u1 _ _ dv_fin IHuv_inf_u0 IHuv_inf_u1 H1 as EVAL. *)
+
+  (*     rewrite IS1.MEM.CP.CONC.concretize_equation; *)
+  (*       red; rewrite IS1.LLVM.MEM.CP.CONCBASE.concretize_uvalueM_equation; *)
+  (*       cbn; repeat red. *)
+
+  (*     specialize (IHuv_inf_u _ H). *)
+
+  (*     exists (ret (fin_to_inf_dvalue x1)). *)
+  (*     exists (fun dv_inf => (fmap fin_to_inf_dvalue (x0 x1))). *)
+  (*     split; eauto. *)
+  (*     split; cbn; rewrite <- Heqx0x1; cbn; eauto. *)
+
+  (*     right. *)
+  (*     intros a ?; subst. *)
+  (*     auto. *)
+  (*   - (* ExtractByte *) *)
+  (*     red; intros dv_fin CONC_FIN. *)
+  (*     red in REF. *)
+  (*     cbn in REF. *)
+  (*     break_match_hyp_inv. *)
+  (*     cbn in *. *)
+  (*     inv CONC_FIN. *)
+  (*   - (* ConcatBytes *) *)
+  (*     cbn in *. *)
+  (*     unfold uvalue_concretize_fin_inf_inclusion in *. *)
+  (*     intros dv_fin H0. *)
+
+  (*     red in REF. *)
+  (*     cbn in REF. *)
+  (*     break_match_hyp_inv. *)
+
+  (*     rewrite IS1.MEM.CP.CONC.concretize_equation; *)
+  (*       red; rewrite IS1.LLVM.MEM.CP.CONCBASE.concretize_uvalueM_equation; *)
+  (*       cbn; repeat red. *)
+
+  (*     admit. *)
+      (* Admitted. *)
+  Abort.
 
   Lemma uvalue_concretize_strict_concretize_inclusion :
     forall uv_inf uv_fin,
@@ -11844,7 +14039,12 @@ Qed.
       uvalue_refine_strict uv_inf uv_fin ->
       uvalue_concretize_inf_fin_inclusion uv_inf uv_fin.
   Proof.
-  Admitted.
+    (* I don't think this is true? *)
+    intros uv_inf uv_fin H.
+    unfold uvalue_concretize_inf_fin_inclusion.
+    intros dv_inf H0.
+    (* dv_inf may not have a finite equivalent *)
+  Abort.
 
   Lemma fin_to_inf_dvalue_injective :
     forall dv1 dv2,
@@ -11858,8 +14058,8 @@ Qed.
       break_match_hyp_inv; clear Heqs; destruct p; clear e1.
       cbn in e.
       break_match_hyp_inv.
-      (* TODO: Need to move dvalue_convert_strict_addr_inv *)
-      admit.
+      epose proof dvalue_convert_strict_addr_inv.
+      specialize (H0 dv2).
   Admitted.
 
   (* Could be the case that OOM happens...
@@ -12148,6 +14348,8 @@ Qed.
     apply fin_to_inf_dvalue_injective in H1;
       subst; auto.
   Qed.
+
+  Print Assumptions uvalue_refine_strict_unique_prop.
 
   Lemma uvalue_refine_strict_non_poison_prop :
     forall uv_inf uv_fin,
